@prefix : <http://ontologies.atb-bremen.de/smashHitCore#> .
@prefix owl: <http://www.w3.org/2002/07/owl#> .
@prefix rdf: <http://www.w3.org/1999/02/22-rdf-syntax-ns#> .
@prefix xml: <http://www.w3.org/XML/1998/namespace> .
@prefix xsd: <http://www.w3.org/2001/XMLSchema#> .
@prefix rdfs: <http://www.w3.org/2000/01/rdf-schema#> .
@base <http://ontologies.atb-bremen.de/smashHitCore> .

<http://ontologies.atb-bremen.de/smashHitCore> rdf:type owl:Ontology ;
                                                owl:versionIRI <http://www.w3.org/2002/07/owl> ;
                                                owl:imports <http://www.w3.org/2000/01/rdf-schema> ;
                                                rdfs:isDefinedBy <http://www.w3.org/TR/owl2-mapping-to-rdf/> ,
                                                                 <http://www.w3.org/TR/owl2-rdf-based-semantics/> ,
                                                                 <http://www.w3.org/TR/owl2-syntax/> ;
                                                rdfs:label "The OWL 2 Schema vocabulary (OWL 2)" ,
                                                           "The RDF Concepts Vocabulary (RDF)" ,
                                                           "The RDF Schema vocabulary (RDFS)" ;
                                                rdfs:seeAlso <http://www.w3.org/2000/01/rdf-schema-more> ,
                                                             <http://www.w3.org/TR/owl2-rdf-based-semantics/#table-axiomatic-classes> ,
                                                             <http://www.w3.org/TR/owl2-rdf-based-semantics/#table-axiomatic-properties> ;
                                                owl:versionInfo "$Date: 2009/11/15 10:54:12 $" ;
                                                <http://www.w3.org/2003/g/data-view#namespaceTransformation> <http://dev.w3.org/cvsweb/2009/owl-grddl/owx2rdf.xsl> .

#################################################################
#    Annotation properties
#################################################################

###  dc:description
<dc:description> rdf:type owl:AnnotationProperty ;
                 rdfs:comment """
Description may include but is not limited to an abstract, a table of contents, a graphical representation, or a free text account of the resource."""@en ;
                 rdfs:domain :license .


###  dcat:bbox
<dcat:bbox> rdfs:comment "The geographic bounding box of a resource."@en ;
            rdf:type owl:AnnotationProperty ;
            rdfs:domain <dct:Location> .


###  dcat:endDate
<dcat:endDate> rdfs:label "The end of the period."@en ;
               rdf:type owl:AnnotationProperty ;
               rdfs:domain <dct:PeriodOfTime> .


###  dcat:startDate
<dcat:startDate> rdfs:comment """The start of the period.
"""@en ;
                 rdf:type owl:AnnotationProperty ;
                 rdfs:domain <dct:PeriodOfTime> .


###  http://creativecommons.org/ns#jurisdiction
<http://creativecommons.org/ns#jurisdiction> rdf:type owl:AnnotationProperty ;
                                             rdfs:domain :license .


###  http://ontologies.atb-bremen.de/context#hasContext
<http://ontologies.atb-bremen.de/context#hasContext> rdfs:label "hasContext"@en ;
                                                     rdf:type owl:AnnotationProperty ;
                                                     rdfs:domain <http://ontologies.atb-bremen.de/context#test_context> .


###  http://ontologies.atb-bremen.de/smashHitCore#ContractProvider
:ContractProvider rdf:type owl:AnnotationProperty .


###  http://ontologies.atb-bremen.de/smashHitCore#ContractRequester
:ContractRequester rdf:type owl:AnnotationProperty .


###  http://ontologies.atb-bremen.de/smashHitCore#contractType
:contractType rdf:type owl:AnnotationProperty .


###  http://ontologies.atb-bremen.de/smashHitCore#hasStreetAddress
:hasStreetAddress rdf:type owl:AnnotationProperty .


###  http://purl.org/dc/elements/1.1/title
<http://purl.org/dc/elements/1.1/title> rdf:type owl:AnnotationProperty .


###  http://www.w3.org/2000/01/rdf-schema#comment
rdfs:comment rdfs:comment "A description of the subject resource." ;
             rdfs:isDefinedBy rdfs: ;
             rdfs:label "comment" ;
             rdfs:range rdfs:Literal ;
             rdfs:domain rdfs:Resource .


###  http://www.w3.org/2000/01/rdf-schema#isDefinedBy
rdfs:isDefinedBy rdfs:subPropertyOf rdfs:seeAlso ;
                 rdfs:range rdfs:Resource ;
                 rdfs:domain rdfs:Resource .


###  http://www.w3.org/2000/01/rdf-schema#label
rdfs:label rdfs:range rdfs:Literal ;
           rdfs:domain rdfs:Resource .


###  http://www.w3.org/2000/01/rdf-schema#seeAlso
rdfs:seeAlso rdfs:range rdfs:Resource ;
             rdfs:domain rdfs:Resource .


###  http://www.w3.org/2002/07/owl#backwardCompatibleWith
owl:backwardCompatibleWith rdf:type owl:AnnotationProperty ;
                           rdfs:comment "The annotation property that indicates that a given ontology is backward compatible with another ontology." ;
                           rdfs:isDefinedBy owl: ;
                           rdfs:label "backwardCompatibleWith" ;
                           rdfs:range owl:Ontology ;
                           rdfs:domain owl:Ontology .


###  http://www.w3.org/2002/07/owl#deprecated
owl:deprecated rdf:type owl:AnnotationProperty ;
               rdfs:comment "The annotation property that indicates that a given entity has been deprecated." ;
               rdfs:isDefinedBy owl: ;
               rdfs:label "deprecated" ;
               rdfs:range rdfs:Resource ;
               rdfs:domain rdfs:Resource .


###  http://www.w3.org/2002/07/owl#imports
owl:imports rdf:type owl:AnnotationProperty ;
            rdfs:comment "The property that is used for importing other ontologies into a given ontology." ;
            rdfs:isDefinedBy owl: ;
            rdfs:label "imports" ;
            rdfs:range owl:Ontology ;
            rdfs:domain owl:Ontology .


###  http://www.w3.org/2002/07/owl#incompatibleWith
owl:incompatibleWith rdf:type owl:AnnotationProperty ;
                     rdfs:comment "The annotation property that indicates that a given ontology is incompatible with another ontology." ;
                     rdfs:isDefinedBy owl: ;
                     rdfs:label "incompatibleWith" ;
                     rdfs:range owl:Ontology ;
                     rdfs:domain owl:Ontology .


###  http://www.w3.org/2002/07/owl#priorVersion
owl:priorVersion rdf:type owl:AnnotationProperty ;
                 rdfs:comment "The annotation property that indicates the predecessor ontology of a given ontology." ;
                 rdfs:isDefinedBy owl: ;
                 rdfs:label "priorVersion" ;
                 rdfs:range owl:Ontology ;
                 rdfs:domain owl:Ontology .


###  http://www.w3.org/2002/07/owl#versionIRI
owl:versionIRI rdf:type owl:AnnotationProperty ;
               rdfs:comment "The property that identifies the version IRI of an ontology." ;
               rdfs:isDefinedBy owl: ;
               rdfs:label "versionIRI" ;
               rdfs:range owl:Ontology ;
               rdfs:domain owl:Ontology .


###  http://www.w3.org/2002/07/owl#versionInfo
owl:versionInfo rdf:type owl:AnnotationProperty ;
                rdfs:range rdfs:Resource ;
                rdfs:domain rdfs:Resource .


###  http://www.w3.org/2003/g/data-view#namespaceTransformation
<http://www.w3.org/2003/g/data-view#namespaceTransformation> rdf:type owl:AnnotationProperty .


###  http://www.w3.org/ns/odrl/2/assignee
<http://www.w3.org/ns/odrl/2/assignee> rdf:type owl:AnnotationProperty ;
                                       rdfs:label "assignee"@en ;
                                       rdfs:range <http://www.w3.org/ns/prov#Agent> ;
                                       rdfs:domain <http://www.w3.org/ns/odrl/2/Policy> .


###  http://www.w3.org/ns/odrl/2/assigner
<http://www.w3.org/ns/odrl/2/assigner> rdf:type owl:AnnotationProperty ;
                                       rdfs:comment "The Party is the issuer of the Rule." ;
                                       rdfs:label "assigner"@en ;
                                       rdfs:range <http://www.w3.org/ns/prov#Agent> ;
                                       rdfs:domain _:genid-nodeid-node1f3qceq4hx1 .


###  http://www.w3.org/ns/odrl/2/duty
<http://www.w3.org/ns/odrl/2/duty> rdf:type owl:AnnotationProperty ;
                                   rdfs:comment """Relates an individual Duty to a Permission.
A Duty is a pre-condition which must be fulfilled in order to receive the Permission."""@en ;
                                   rdfs:label "hasDuty"@en ;
                                   rdfs:range <http://www.w3.org/ns/odrl/2/Duty> ;
                                   rdfs:domain <http://www.w3.org/ns/odrl/2/Permission> .


###  http://www.w3.org/ns/odrl/2/hasAction
<http://www.w3.org/ns/odrl/2/hasAction> rdf:type owl:AnnotationProperty ;
                                        rdfs:comment "\"The operation relating to the Asset for which the Rule is being subjected.\""@en ;
                                        rdfs:label "hasAction"@en ;
                                        rdfs:domain <http://www.w3.org/ns/odrl/2/Policy> .


###  https://dalicc.poolparty.biz/DALICC/LiabilityLimitation
<https://dalicc.poolparty.biz/DALICC/LiabilityLimitation> rdf:type owl:AnnotationProperty ;
                                                          rdfs:domain :license .


###  https://dalicc.poolparty.biz/DALICC/WarrantyDisclaimer
<https://dalicc.poolparty.biz/DALICC/WarrantyDisclaimer> rdf:type owl:AnnotationProperty ;
                                                         rdfs:domain :license .


###  https://dalicc.poolparty.biz/DALICC/WarrantyOrLiabilityAcceptance
<https://dalicc.poolparty.biz/DALICC/WarrantyOrLiabilityAcceptance> rdf:type owl:AnnotationProperty ;
                                                                    rdfs:domain :license .


###  https://dalicc.poolparty.biz/DALICC/additionalClauses
<https://dalicc.poolparty.biz/DALICC/additionalClauses> rdf:type owl:AnnotationProperty ;
                                                        rdfs:domain :license .


#################################################################
#    Datatypes
#################################################################

###  http://www.w3.org/1999/02/22-rdf-syntax-ns#HTML
rdf:HTML rdf:type rdfs:Datatype .


###  http://www.w3.org/1999/02/22-rdf-syntax-ns#XMLLiteral
rdf:XMLLiteral rdf:type rdfs:Datatype .


###  https://www.w3.org/TR/xmlschema11-2/#dateTimeStamp
<https://www.w3.org/TR/xmlschema11-2/#dateTimeStamp> rdf:type rdfs:Datatype ;
                                                     rdfs:label "dateTimeStamp"@en .


#################################################################
#    Object Properties
#################################################################

###  dpv:hasPersonalDataCategory
<dpv:hasPersonalDataCategory> rdf:type owl:ObjectProperty ;
                              rdfs:range <http://www.w3.org/ns/dpv#PersonalDataCategory> ;
                              rdfs:comment "This property associates a personal data category with an instance of legal data handling or consent"@en ;
                              rdfs:label "has personal data category"@en .


###  fibo-der-drc-ma:hasBeneficiary
<fibo-der-drc-ma:hasBeneficiary> rdf:type owl:ObjectProperty ;
                                 rdfs:domain <https://spec.edmcouncil.org/fibo/ontology/FND/Agreements/Contracts/Contract_> ;
                                 rdfs:range <https://spec.edmcouncil.org/fibo/ontology/DER/DerivativesContracts/DerivativesMasterAgreements/CreditSupportAgreement> ;
                                 rdfs:comment "Has beneficiary is a kind of has counterparty."@en ;
                                 rdfs:label "hasBeneficiary"@en .


###  fibo-fnd-agr-ctr:isAssignable
<fibo-fnd-agr-ctr:isAssignable> rdf:type owl:ObjectProperty ;
                                rdfs:domain <https://spec.edmcouncil.org/fibo/ontology/FND/Agreements/Contracts/Contract_> ;
                                rdfs:range <fibo-fbc-fi-fi:NegotiableSecurity> ,
                                           <fibo-fnd-agr-ctr:AssignableContract> ,
                                           <fibo-fnd-agr-ctr:NovateableContract> ;
                                rdfs:comment "Specifies whether a particular financial instrument is or is not transferable"@en ;
                                rdfs:label "isAssignable"@en .


###  http://ontologies.atb-bremen.de/smashHitCore#GrantedAtTime
:GrantedAtTime rdf:type owl:ObjectProperty ;
               rdfs:subPropertyOf :hasStatus ;
               rdf:type owl:FunctionalProperty ;
               rdfs:domain :ConsentID ;
               rdfs:range :Granted .


###  http://ontologies.atb-bremen.de/smashHitCore#RevokedAtTime
:RevokedAtTime rdf:type owl:ObjectProperty ;
               rdfs:subPropertyOf :hasStatus ;
               rdf:type owl:FunctionalProperty ;
               rdfs:domain :ConsentID ;
               rdfs:range :Revoked .


###  http://ontologies.atb-bremen.de/smashHitCore#atCity
:atCity rdf:type owl:ObjectProperty ;
        rdfs:subPropertyOf :atLocation ;
        rdf:type owl:FunctionalProperty ;
        rdfs:domain <http://purl.org/adaptcentre/openscience/ontologies/consent#Context> ;
        rdfs:range :City .


###  http://ontologies.atb-bremen.de/smashHitCore#atCountry
:atCountry rdf:type owl:ObjectProperty ;
           rdfs:subPropertyOf :atLocation ;
           rdf:type owl:FunctionalProperty ;
           rdfs:domain <http://purl.org/adaptcentre/openscience/ontologies/consent#Location> ;
           rdfs:range :Country .


###  http://ontologies.atb-bremen.de/smashHitCore#atDateTime
:atDateTime rdf:type owl:ObjectProperty ;
            rdfs:subPropertyOf :hasContext ;
            rdf:type owl:FunctionalProperty ;
            rdfs:domain :ConsentID ,
                        rdf:Status ;
            rdfs:range <http://purl.org/adaptcentre/openscience/ontologies/consent#Time> .


###  http://ontologies.atb-bremen.de/smashHitCore#atLocation
:atLocation rdf:type owl:ObjectProperty ;
            rdfs:subPropertyOf :hasContext ;
            rdfs:domain :consent ;
            rdfs:range <http://purl.org/adaptcentre/openscience/ontologies/consent#Location> .


###  http://ontologies.atb-bremen.de/smashHitCore#atRegion
:atRegion rdf:type owl:ObjectProperty ;
          rdfs:subPropertyOf :atLocation ;
          rdf:type owl:FunctionalProperty ;
          rdfs:domain <http://purl.org/adaptcentre/openscience/ontologies/consent#Location> ;
          rdfs:range :Region .


###  http://ontologies.atb-bremen.de/smashHitCore#atState
:atState rdf:type owl:ObjectProperty ;
         rdfs:subPropertyOf :atLocation ;
         rdf:type owl:FunctionalProperty ;
         rdfs:domain <http://purl.org/adaptcentre/openscience/ontologies/consent#Location> ;
         rdfs:range :State .


###  http://ontologies.atb-bremen.de/smashHitCore#forDataProcessing
:forDataProcessing rdf:type owl:ObjectProperty ,
                            owl:FunctionalProperty ;
                   rdfs:range rdf:Data_Processing .


###  http://ontologies.atb-bremen.de/smashHitCore#forPurpose
:forPurpose rdf:type owl:ObjectProperty ,
                     owl:SymmetricProperty ;
            rdfs:domain :consent .


###  http://ontologies.atb-bremen.de/smashHitCore#hasAddress
:hasAddress rdf:type owl:ObjectProperty ;
            rdfs:domain <https://spec.edmcouncil.org/fibo/ontology/FND/Agreements/Contracts/Contract_> ;
            rdfs:range <fibo-fnd-plc-adr:Address> ;
            rdfs:comment "Specify the physical address of a location."@en ;
            rdfs:label "hasAddress"@en .


###  http://ontologies.atb-bremen.de/smashHitCore#hasAmendment
:hasAmendment rdf:type owl:ObjectProperty ;
              rdfs:domain <https://spec.edmcouncil.org/fibo/ontology/FND/Agreements/Contracts/Contract_> ;
              rdfs:range <https://spec.edmcouncil.org/fibo/ontology/FND/Agreements/Contracts/ContractDocument> .


###  http://ontologies.atb-bremen.de/smashHitCore#hasAssociation
:hasAssociation rdf:type owl:ObjectProperty ;
                rdfs:domain :consent ,
                            :metadata ,
                            rdf:Data_Processing ,
                            <https://spec.edmcouncil.org/fibo/ontology/FND/Agreements/Contracts/Contract_> ;
                rdfs:range owl:Thing ;
                rdfs:comment "Indicates and Association with another entity for a Purpose or Data Processing."@en .


###  http://ontologies.atb-bremen.de/smashHitCore#hasCity
:hasCity rdf:type owl:ObjectProperty ;
         rdfs:subPropertyOf :hasContractLocation ;
         rdfs:domain <https://spec.edmcouncil.org/fibo/ontology/FND/Agreements/Contracts/Contract_> .


###  http://ontologies.atb-bremen.de/smashHitCore#hasConfidentialityObligation
:hasConfidentialityObligation rdf:type owl:ObjectProperty ;
                              rdfs:domain <https://spec.edmcouncil.org/fibo/ontology/FND/Agreements/Contracts/Contract_> ;
                              rdfs:range <https://spec.edmcouncil.org/fibo/ontology/FND/Agreements/Contracts/ContractDocument> .


###  http://ontologies.atb-bremen.de/smashHitCore#hasContext
:hasContext rdf:type owl:ObjectProperty ,
                     owl:FunctionalProperty ;
            rdfs:domain :consent ;
            rdfs:range <http://purl.org/adaptcentre/openscience/ontologies/consent#Context> ;
            rdfs:comment "Links a consent instance to the context in which it was acquired/provided/given."@en .


###  http://ontologies.atb-bremen.de/smashHitCore#hasContractLocation
:hasContractLocation rdf:type owl:ObjectProperty .


###  http://ontologies.atb-bremen.de/smashHitCore#hasContractStatus
:hasContractStatus rdf:type owl:ObjectProperty ;
                   rdfs:domain <https://spec.edmcouncil.org/fibo/ontology/FND/Agreements/Contracts/Contract_> .


###  http://ontologies.atb-bremen.de/smashHitCore#hasContractType
:hasContractType rdf:type owl:ObjectProperty ;
                 rdfs:domain <https://spec.edmcouncil.org/fibo/ontology/FND/Agreements/Contracts/Contract_> ;
                 rdfs:range <https://spec.edmcouncil.org/fibo/ontology/FND/Agreements/Contracts/Contract_> ;
                 rdfs:comment "It specify the different type of contracts such as Written Contract, Credit Support Agreement, Verbal contract etc."@en ;
                 rdfs:label "hasContractType"@en .


###  http://ontologies.atb-bremen.de/smashHitCore#hasCountry
:hasCountry rdf:type owl:ObjectProperty ;
            rdfs:subPropertyOf :hasContractLocation ;
            rdfs:domain <https://spec.edmcouncil.org/fibo/ontology/FND/Agreements/Contracts/Contract_> .


###  http://ontologies.atb-bremen.de/smashHitCore#hasDataController
:hasDataController rdf:type owl:ObjectProperty ;
                   rdfs:domain :consent ,
                               :contract ,
                               <https://spec.edmcouncil.org/fibo/ontology/FND/Agreements/Contracts/Contract_> ;
                   rdfs:range <http://www.w3.org/ns/prov#Agent> .


###  http://ontologies.atb-bremen.de/smashHitCore#hasDataProtection
:hasDataProtection rdf:type owl:ObjectProperty ;
                   rdfs:domain <https://spec.edmcouncil.org/fibo/ontology/FND/Agreements/Contracts/Contract_> ;
                   rdfs:range <https://spec.edmcouncil.org/fibo/ontology/FND/Agreements/Contracts/ContractDocument> .


###  http://ontologies.atb-bremen.de/smashHitCore#hasEmail
:hasEmail rdf:type owl:ObjectProperty ,
                   owl:FunctionalProperty ;
          rdfs:domain <http://www.w3.org/2004/02/skos/core#Concept> ,
                      <http://www.w3.org/ns/dpv#Name> ,
                      <http://www.w3.org/ns/prov#Agent> ;
          rdfs:range <http://www.w3.org/ns/dpv#EmailAddress> .


###  http://ontologies.atb-bremen.de/smashHitCore#hasExpirationDate
:hasExpirationDate rdf:type owl:ObjectProperty ;
                   rdfs:subPropertyOf :hasContext ;
                   rdf:type owl:FunctionalProperty ;
                   rdfs:domain :ConsentID ,
                               rdf:Status ;
                   rdfs:range :ExpirationDate ;
                   rdfs:comment "The expiration date of consent or contract. Format: xsd:dateTime"@en ;
                   rdfs:label "ExpirationDate"@en .


###  http://ontologies.atb-bremen.de/smashHitCore#hasExpiry
:hasExpiry rdf:type owl:ObjectProperty ,
                    owl:FunctionalProperty ;
           rdfs:domain :consent ,
                       <https://spec.edmcouncil.org/fibo/ontology/FND/Agreements/Contracts/Contract_> ;
           rdfs:comment """Specifies the Instant or Duration in which the consent expires.
"""@en .


###  http://ontologies.atb-bremen.de/smashHitCore#hasHash
:hasHash rdf:type owl:ObjectProperty ,
                  owl:FunctionalProperty ;
         rdfs:domain :SensorDataCategory ,
                     rdf:Data_Processing ,
                     <http://www.w3.org/ns/dcat#Resource> ;
         rdfs:range :Hash .


###  http://ontologies.atb-bremen.de/smashHitCore#hasLimitationOnUse
:hasLimitationOnUse rdf:type owl:ObjectProperty ;
                    rdfs:domain <https://spec.edmcouncil.org/fibo/ontology/FND/Agreements/Contracts/Contract_> ;
                    rdfs:range <https://spec.edmcouncil.org/fibo/ontology/FND/Agreements/Contracts/ContractDocument> .


###  http://ontologies.atb-bremen.de/smashHitCore#hasMetadata
:hasMetadata rdf:type owl:ObjectProperty ;
             rdfs:domain <http://www.w3.org/ns/dcat#Resource> ;
             rdfs:range :metadata ;
             rdfs:comment "Links the Resource to the metadata"@en .


###  http://ontologies.atb-bremen.de/smashHitCore#hasMethodOfNotice
:hasMethodOfNotice rdf:type owl:ObjectProperty ;
                   rdfs:domain <https://spec.edmcouncil.org/fibo/ontology/FND/Agreements/Contracts/Contract_> ;
                   rdfs:range <https://spec.edmcouncil.org/fibo/ontology/FND/Agreements/Contracts/ContractDocument> .


###  http://ontologies.atb-bremen.de/smashHitCore#hasMinimumDuration
:hasMinimumDuration rdf:type owl:ObjectProperty ;
                    rdfs:domain <https://spec.edmcouncil.org/fibo/ontology/FND/Agreements/Contracts/Contract_> .


###  http://ontologies.atb-bremen.de/smashHitCore#hasName
:hasName rdf:type owl:ObjectProperty ;
         rdfs:domain <http://www.w3.org/2004/02/skos/core#Concept> ,
                     <http://www.w3.org/ns/prov#Agent> ;
         rdfs:range <http://www.w3.org/ns/dpv#Name> .


###  http://ontologies.atb-bremen.de/smashHitCore#hasNoThirdPartyBeneficiaries
:hasNoThirdPartyBeneficiaries rdf:type owl:ObjectProperty ;
                              rdfs:domain <https://spec.edmcouncil.org/fibo/ontology/FND/Agreements/Contracts/Contract_> ;
                              rdfs:range <https://spec.edmcouncil.org/fibo/ontology/FND/Agreements/Contracts/ContractDocument> .


###  http://ontologies.atb-bremen.de/smashHitCore#hasPermittedDisclosure
:hasPermittedDisclosure rdf:type owl:ObjectProperty ;
                        rdfs:domain <https://spec.edmcouncil.org/fibo/ontology/FND/Agreements/Contracts/Contract_> ;
                        rdfs:range <https://spec.edmcouncil.org/fibo/ontology/FND/Agreements/Contracts/ContractDocument> .


###  http://ontologies.atb-bremen.de/smashHitCore#hasPersonalData
:hasPersonalData rdf:type owl:ObjectProperty ,
                          owl:FunctionalProperty ;
                 rdfs:domain <http://www.w3.org/ns/dpv#PersonalDataCategory> ,
                             <http://www.w3.org/ns/prov#Agent> ;
                 rdfs:range <http://www.w3.org/ns/dpv#PersonalDataCategory> .


###  http://ontologies.atb-bremen.de/smashHitCore#hasPostalCode
:hasPostalCode rdf:type owl:ObjectProperty ;
               rdfs:subPropertyOf :hasContractLocation ;
               rdfs:domain <https://spec.edmcouncil.org/fibo/ontology/FND/Agreements/Contracts/Contract_> .


###  http://ontologies.atb-bremen.de/smashHitCore#hasPurposePreference
:hasPurposePreference rdf:type owl:ObjectProperty ;
                      rdfs:domain <http://www.w3.org/ns/prov#Agent> ;
                      rdfs:range <http://www.w3.org/ns/dpv#Purpose> .


###  http://ontologies.atb-bremen.de/smashHitCore#hasReceiptOfNotice
:hasReceiptOfNotice rdf:type owl:ObjectProperty ;
                    rdfs:domain <https://spec.edmcouncil.org/fibo/ontology/FND/Agreements/Contracts/Contract_> ;
                    rdfs:range <https://spec.edmcouncil.org/fibo/ontology/FND/Agreements/Contracts/ContractDocument> .


###  http://ontologies.atb-bremen.de/smashHitCore#hasRole
:hasRole rdf:type owl:ObjectProperty ;
         rdfs:domain <http://www.w3.org/ns/prov#Agent> ;
         rdfs:range <http://www.w3.org/ns/dcat#Role> .


###  http://ontologies.atb-bremen.de/smashHitCore#hasSensorDataCategory
:hasSensorDataCategory rdf:type owl:ObjectProperty ;
                       rdfs:domain :SensorData ;
                       rdfs:range :SensorDataCategory .


###  http://ontologies.atb-bremen.de/smashHitCore#hasSeverability
:hasSeverability rdf:type owl:ObjectProperty ;
                 rdfs:domain <https://spec.edmcouncil.org/fibo/ontology/FND/Agreements/Contracts/Contract_> ;
                 rdfs:range <https://spec.edmcouncil.org/fibo/ontology/FND/Agreements/Contracts/ContractDocument> .


###  http://ontologies.atb-bremen.de/smashHitCore#hasStatus
:hasStatus rdf:type owl:ObjectProperty ,
                    owl:FunctionalProperty ;
           rdfs:domain :ConsentID ;
           rdfs:range :ConsentStatus .


###  http://ontologies.atb-bremen.de/smashHitCore#hasTelephone
:hasTelephone rdf:type owl:ObjectProperty ,
                       owl:FunctionalProperty ;
              rdfs:domain <http://www.w3.org/ns/prov#Agent> ;
              rdfs:range :TelephoneNumber .


###  http://ontologies.atb-bremen.de/smashHitCore#hasTerminationForInsolvency
:hasTerminationForInsolvency rdf:type owl:ObjectProperty ;
                             rdfs:domain <https://spec.edmcouncil.org/fibo/ontology/FND/Agreements/Contracts/Contract_> ;
                             rdfs:range <https://spec.edmcouncil.org/fibo/ontology/FND/Agreements/Contracts/ContractDocument> .


###  http://ontologies.atb-bremen.de/smashHitCore#hasTerminationForMaterialBreach
:hasTerminationForMaterialBreach rdf:type owl:ObjectProperty ;
                                 rdfs:domain <https://spec.edmcouncil.org/fibo/ontology/FND/Agreements/Contracts/Contract_> ;
                                 rdfs:range <https://spec.edmcouncil.org/fibo/ontology/FND/Agreements/Contracts/ContractDocument> .


###  http://ontologies.atb-bremen.de/smashHitCore#hasTerminationOnNotice
:hasTerminationOnNotice rdf:type owl:ObjectProperty ;
                        rdfs:domain <https://spec.edmcouncil.org/fibo/ontology/FND/Agreements/Contracts/Contract_> ;
                        rdfs:range <https://spec.edmcouncil.org/fibo/ontology/FND/Agreements/Contracts/ContractDocument> .


###  http://ontologies.atb-bremen.de/smashHitCore#hasUsername
:hasUsername rdf:type owl:ObjectProperty ;
             rdfs:subPropertyOf :hasPersonalData ;
             rdf:type owl:FunctionalProperty ;
             rdfs:domain <http://www.w3.org/ns/prov#Agent> ;
             rdfs:range <http://www.w3.org/ns/dpv#Username> .


###  http://ontologies.atb-bremen.de/smashHitCore#hasWaiver
:hasWaiver rdf:type owl:ObjectProperty ;
           rdfs:domain <https://spec.edmcouncil.org/fibo/ontology/FND/Agreements/Contracts/Contract_> ;
           rdfs:range <https://spec.edmcouncil.org/fibo/ontology/FND/Agreements/Contracts/ContractDocument> .


###  http://ontologies.atb-bremen.de/smashHitCore#inMedium
:inMedium rdf:type owl:ObjectProperty ;
          rdfs:subPropertyOf :hasContext ;
          rdfs:domain :consent ;
          rdfs:range <https://w3id.org/GConsent#Medium> ;
          rdfs:comment """
Specifies the medium through which the consent was given. Examples are web forms, paper documents.
"""@en .


###  http://ontologies.atb-bremen.de/smashHitCore#isAboutData
:isAboutData rdf:type owl:ObjectProperty ;
             rdfs:domain :ConsentID ;
             rdfs:range :SensorDataCategory ,
                        :metadata ,
                        rdf:Data_Processing ,
                        <http://www.w3.org/ns/dcat#Resource> .


###  http://ontologies.atb-bremen.de/smashHitCore#isProvidedBy
:isProvidedBy rdf:type owl:ObjectProperty ,
                       owl:FunctionalProperty ,
                       owl:AsymmetricProperty ,
                       owl:IrreflexiveProperty ;
              rdfs:domain :consent ;
              rdfs:range rdf:Status ,
                         <http://www.w3.org/ns/dpv#PersonalDataCategory> ,
                         <http://www.w3.org/ns/prov#Agent> ;
              rdfs:comment """
Indicates the entity or activitiy that provided the consent.
"""@en .


###  http://ontologies.atb-bremen.de/smashHitCore#requestedBy
:requestedBy rdf:type owl:ObjectProperty ,
                      owl:FunctionalProperty ;
             rdfs:domain :consent ;
             rdfs:range <http://www.w3.org/ns/prov#Agent> .


###  http://ontologies.atb-bremen.de/smashHitCore#unit
:unit rdf:type owl:ObjectProperty .


###  http://ontologies.atb-bremen.de/smashHitCore#value
:value rdf:type owl:ObjectProperty .


###  http://purl.org/adaptcentre/openscience/ontologies/consent#data_has_a_format
<http://purl.org/adaptcentre/openscience/ontologies/consent#data_has_a_format> rdf:type owl:ObjectProperty ;
                                                                               rdfs:range <http://purl.org/adaptcentre/openscience/ontologies/consent#ConsentFormat> ;
                                                                               rdfs:label "data_has_format"@en .


###  http://purl.org/dc/terms/accessRights
<http://purl.org/dc/terms/accessRights> rdf:type owl:ObjectProperty ;
                                        rdfs:domain <http://www.w3.org/ns/dcat#Resource> ;
                                        rdfs:comment "A rights statement that concerns how the distribution is accessed."@en .


###  http://purl.org/dc/terms/format
<http://purl.org/dc/terms/format> rdf:type owl:ObjectProperty ;
                                  rdfs:domain <http://www.w3.org/ns/dcat#Resource> ;
                                  rdfs:comment "The file format of the distribution."@en .


###  http://purl.org/dc/terms/hasVersion
<http://purl.org/dc/terms/hasVersion> rdf:type owl:ObjectProperty ,
                                               owl:FunctionalProperty ,
                                               owl:TransitiveProperty ;
                                      rdfs:domain :consent ;
                                      rdfs:range :consent ,
                                                 rdf:Status ;
                                      rdfs:comment """A related resource that is a version, edition, or adaptation of the described resource.
Can be the version of consent and/or contract."""@en .


###  http://purl.org/dc/terms/identifier
<http://purl.org/dc/terms/identifier> rdf:type owl:ObjectProperty ,
                                               owl:FunctionalProperty ;
                                      rdfs:domain :consent ,
                                                  <http://www.w3.org/ns/dcat#Resource> ;
                                      rdfs:range :ConsentID ;
                                      rdfs:comment "A unique identifier of the item."@en .


###  http://purl.org/dc/terms/language
<http://purl.org/dc/terms/language> rdf:type owl:ObjectProperty ;
                                    rdfs:domain <http://www.w3.org/ns/dcat#Resource> ;
                                    rdfs:comment "A language of the item. This refers to the natural language used for textual metadata (i.e. titles, descriptions, etc) of a cataloged resource (i.e. dataset or service) or the textual values of a dataset distribution"@en .


###  http://purl.org/dc/terms/modified
<http://purl.org/dc/terms/modified> rdf:type owl:ObjectProperty ;
                                    rdfs:domain <http://www.w3.org/ns/dcat#Resource> ;
                                    rdfs:comment "Most recent date on which the distribution was changed, updated or modified."@en .


###  http://purl.org/dc/terms/rights
<http://purl.org/dc/terms/rights> rdf:type owl:ObjectProperty ;
                                  rdfs:domain <http://www.w3.org/ns/dcat#Resource> ;
                                  rdfs:comment "Information about rights held in and over the distribution."@en .


###  http://purl.org/dc/terms/title
<http://purl.org/dc/terms/title> rdf:type owl:ObjectProperty ;
                                 rdfs:domain <http://www.w3.org/ns/dcat#Resource> ;
                                 rdfs:comment "A name given to the distribution."@en .


###  http://purl.org/dc/terms/type
<http://purl.org/dc/terms/type> rdf:type owl:ObjectProperty ;
                                rdfs:domain <http://www.w3.org/ns/dcat#Resource> ;
                                rdfs:comment "The nature or genre of the resource."@en .


###  http://www.w3.org/1999/02/22-rdf-syntax-ns#hasInputData
rdf:hasInputData rdf:type owl:ObjectProperty ,
                          owl:SymmetricProperty ,
                          owl:TransitiveProperty ;
                 rdfs:domain rdf:Data_Processing ,
                             <https://spec.edmcouncil.org/fibo/ontology/FND/Agreements/Contracts/Contract_> ;
                 rdfs:range :SensorDataCategory ,
                            <http://www.w3.org/ns/dcat#Resource> .


###  http://www.w3.org/1999/02/22-rdf-syntax-ns#hasOutputData
rdf:hasOutputData rdf:type owl:ObjectProperty ;
                  rdfs:domain rdf:Data_Processing ,
                              <https://spec.edmcouncil.org/fibo/ontology/FND/Agreements/Contracts/Contract_> ;
                  rdfs:range :SensorDataCategory ,
                             <http://www.w3.org/ns/dcat#Resource> .


###  http://www.w3.org/1999/02/22-rdf-syntax-ns#hasType
rdf:hasType rdf:type owl:ObjectProperty ;
            rdfs:domain <http://www.w3.org/ns/prov#Agent> ;
            rdfs:range <http://www.w3.org/ns/prov#Agent> .


###  http://www.w3.org/2002/07/owl#bottomObjectProperty
owl:bottomObjectProperty rdf:type owl:ObjectProperty ;
                         rdfs:domain owl:Thing ;
                         rdfs:range owl:Thing ;
                         rdfs:comment "The object property that does not relate any two individuals." ;
                         rdfs:isDefinedBy owl: ;
                         rdfs:label "bottomObjectProperty" .


###  http://www.w3.org/2002/07/owl#differentFrom
owl:differentFrom rdf:type owl:ObjectProperty ;
                  rdfs:domain owl:Thing ;
                  rdfs:range owl:Thing ;
                  rdfs:comment "The property that determines that two given individuals are different." ;
                  rdfs:isDefinedBy owl: ;
                  rdfs:label "differentFrom" .


###  http://www.w3.org/2002/07/owl#sameAs
owl:sameAs rdf:type owl:ObjectProperty ;
           rdfs:domain owl:Thing ;
           rdfs:range owl:Thing ;
           rdfs:comment "The property that determines that two given individuals are equal." ;
           rdfs:isDefinedBy owl: ;
           rdfs:label "sameAs" .


###  http://www.w3.org/2002/07/owl#sourceIndividual
owl:sourceIndividual rdf:type owl:ObjectProperty ;
                     rdfs:range owl:Thing ;
                     rdfs:comment "The property that determines the subject of a negative property assertion." ;
                     rdfs:isDefinedBy owl: ;
                     rdfs:label "sourceIndividual" .


###  http://www.w3.org/2002/07/owl#targetIndividual
owl:targetIndividual rdf:type owl:ObjectProperty ;
                     rdfs:range owl:Thing ;
                     rdfs:comment "The property that determines the object of a negative object property assertion." ;
                     rdfs:isDefinedBy owl: ;
                     rdfs:label "targetIndividual" .


###  http://www.w3.org/2002/07/owl#topObjectProperty
owl:topObjectProperty rdf:type owl:ObjectProperty ;
                      rdfs:domain owl:Thing ;
                      rdfs:range owl:Thing ;
                      rdfs:comment "The object property that relates every two individuals." ;
                      rdfs:isDefinedBy owl: ;
                      rdfs:label "topObjectProperty" .


###  http://www.w3.org/ns/dcat#bbox
<http://www.w3.org/ns/dcat#bbox> rdf:type owl:ObjectProperty ;
                                 rdfs:domain <http://purl.org/dc/terms/Location> ;
                                 rdfs:comment "The geographic bounding box of a resource."@en .


###  http://www.w3.org/ns/dcat#endDate
<http://www.w3.org/ns/dcat#endDate> rdf:type owl:ObjectProperty ;
                                    rdfs:domain <http://purl.org/dc/terms/PeriodOfTime> .


###  http://www.w3.org/ns/dcat#hadRole
<http://www.w3.org/ns/dcat#hadRole> rdf:type owl:ObjectProperty ;
                                    rdfs:comment "The function of an entity or agent with respect to another entity or resource."@en ;
                                    rdfs:label "hadRole"@en .


###  http://www.w3.org/ns/dcat#startDate
<http://www.w3.org/ns/dcat#startDate> rdf:type owl:ObjectProperty ;
                                      rdfs:domain <http://purl.org/dc/terms/PeriodOfTime> .


###  http://www.w3.org/ns/dcat#theme
<http://www.w3.org/ns/dcat#theme> rdf:type owl:ObjectProperty ;
                                  rdfs:domain <http://www.w3.org/ns/dcat#Resource> ;
                                  rdfs:comment "A main category of the resource. A resource can have multiple themes."@en .


###  http://www.w3.org/ns/dpv#hasPersonalDataCategory
<http://www.w3.org/ns/dpv#hasPersonalDataCategory> rdf:type owl:ObjectProperty ;
                                                   rdfs:range <http://www.w3.org/ns/dpv#PersonalDataCategory> ;
                                                   rdfs:comment "This property associates a personal data category with an instance of legal data handling or consent"@en ;
                                                   rdfs:label "has personal data category"@en .


###  http://www.w3.org/ns/dpv#hasPurpose
<http://www.w3.org/ns/dpv#hasPurpose> rdf:type owl:ObjectProperty ;
                                      rdfs:domain :consent ;
                                      rdfs:range <http://www.w3.org/ns/dpv#Purpose> ;
                                      rdfs:comment "This property associates a purpose with an instance of legal data handling or consent"@en ;
                                      rdfs:label "has Purpose"@en .


###  http://www.w3.org/ns/prov#actedOnBehalfOf
<http://www.w3.org/ns/prov#actedOnBehalfOf> rdf:type owl:ObjectProperty ;
                                            rdfs:subPropertyOf <http://www.w3.org/ns/prov#wasInfluencedBy> ;
                                            rdfs:comment "An object property to express the accountability of an agent towards another agent. The subordinate agent acted on behalf of the responsible agent in an actual activity. "@en ;
                                            rdfs:label "actedOnBehalfOf"@en .


###  http://www.w3.org/ns/prov#wasInfluencedBy
<http://www.w3.org/ns/prov#wasInfluencedBy> rdf:type owl:ObjectProperty ;
                                            rdfs:comment "Because prov:wasInfluencedBy is a broad relation, its more specific subproperties (e.g. prov:wasInformedBy, prov:actedOnBehalfOf, prov:wasEndedBy, etc.) should be used when applicable."@en ;
                                            rdfs:label "wasInfluencedBy"@en .


###  https://schema.org/identifier
<https://schema.org/identifier> rdf:type owl:ObjectProperty ,
                                         owl:FunctionalProperty ;
                                rdfs:domain :consent ;
                                rdfs:range :ConsentID ;
                                rdfs:comment "The identifier property represents any kind of identifier for any kind of Thing, such as ISBNs, GTIN codes, UUIDs etc. Schema.org provides dedicated properties for representing many of these, either as textual strings or as URL (URI) links."@en ;
                                rdfs:label "Identifier "@en .


###  https://spec.edmcouncil.org/fibo/ontology/FND/Agreements/Contracts/hasContractParty
<https://spec.edmcouncil.org/fibo/ontology/FND/Agreements/Contracts/hasContractParty> rdf:type owl:ObjectProperty ;
                                                                                      rdfs:domain <https://spec.edmcouncil.org/fibo/ontology/FND/Agreements/Contracts/Contract_> ;
                                                                                      rdfs:range <http://www.w3.org/ns/prov#Agent> ;
                                                                                      rdfs:comment "Legally competent party that has entered into a binding agreement, accepting and conceding obligations, responsibilities, and benefits as specified" ;
                                                                                      rdfs:label "hasContractParty"@en .


###  https://spec.edmcouncil.org/fibo/ontology/FND/Agreements/Contracts/hasContractualElement
<https://spec.edmcouncil.org/fibo/ontology/FND/Agreements/Contracts/hasContractualElement> rdf:type owl:ObjectProperty ;
                                                                                           rdfs:domain <https://spec.edmcouncil.org/fibo/ontology/FND/Agreements/Contracts/Contract_> ;
                                                                                           rdfs:comment "indicates something that is a component of an agreement"@en ;
                                                                                           rdfs:label "hasContractualElement"@en .


###  https://spec.edmcouncil.org/fibo/ontology/FND/Agreements/Contracts/hasEffectiveDate
<https://spec.edmcouncil.org/fibo/ontology/FND/Agreements/Contracts/hasEffectiveDate> rdf:type owl:ObjectProperty ;
                                                                                      rdfs:domain <https://spec.edmcouncil.org/fibo/ontology/FND/Agreements/Contracts/Contract_> .


###  https://spec.edmcouncil.org/fibo/ontology/FND/Agreements/Contracts/hasEffectiveDateTimeStamp
<https://spec.edmcouncil.org/fibo/ontology/FND/Agreements/Contracts/hasEffectiveDateTimeStamp> rdf:type owl:ObjectProperty ;
                                                                                               rdfs:domain <https://spec.edmcouncil.org/fibo/ontology/FND/Agreements/Contracts/Contract_> ;
                                                                                               rdfs:comment "indicates the date and time, including time zone, something comes into force"@en ;
                                                                                               rdfs:label "hasEffectiveDateTimeStamp"@en .


###  https://spec.edmcouncil.org/fibo/ontology/FND/Agreements/Contracts/hasExecutionDate
<https://spec.edmcouncil.org/fibo/ontology/FND/Agreements/Contracts/hasExecutionDate> rdf:type owl:ObjectProperty ;
                                                                                      rdfs:domain <https://spec.edmcouncil.org/fibo/ontology/FND/Agreements/Contracts/Contract_> .


###  https://spec.edmcouncil.org/fibo/ontology/FND/Agreements/Contracts/hasExecutionDateTimeStamp
<https://spec.edmcouncil.org/fibo/ontology/FND/Agreements/Contracts/hasExecutionDateTimeStamp> rdf:type owl:ObjectProperty ;
                                                                                               rdfs:domain <https://spec.edmcouncil.org/fibo/ontology/FND/Agreements/Contracts/Contract_> ;
                                                                                               rdfs:comment "indicates the date and time, including time zone, a contract has been signed by all the necessary parties"@en ;
                                                                                               rdfs:label "hasExecutionDateTimeStamp"@en .


###  https://w3id.org/GConsent#hasRole
<https://w3id.org/GConsent#hasRole> rdf:type owl:ObjectProperty ,
                                             owl:FunctionalProperty ;
                                    rdfs:domain <http://www.w3.org/ns/prov#Agent> ;
                                    rdfs:range <http://www.w3.org/ns/dcat#Role> ;
                                    rdfs:label "hasRole"@en .


###  https://w3id.org/GConsent#isStatusForConsent
<https://w3id.org/GConsent#isStatusForConsent> rdf:type owl:ObjectProperty ,
                                                        owl:InverseFunctionalProperty ;
                                               rdfs:domain :ConsentStatus ;
                                               rdfs:range :ConsentID ;
                                               rdfs:comment "Links a status to the consent that uses it."@en ;
                                               rdfs:label "isStatusFor"@en .


#################################################################
#    Data properties
#################################################################

###  http://ontologies.atb-bremen.de/smashHitCore#hasID
:hasID rdf:type owl:DatatypeProperty ,
                owl:FunctionalProperty ;
       rdfs:domain <http://www.w3.org/ns/prov#Agent> ;
       rdfs:range rdf:langString .


###  http://www.w3.org/2002/07/owl#bottomDataProperty
owl:bottomDataProperty rdf:type owl:DatatypeProperty ;
                       rdfs:domain owl:Thing ;
                       rdfs:range rdfs:Literal ;
                       rdfs:comment "The data property that does not relate any individual to any data value." ;
                       rdfs:isDefinedBy owl: ;
                       rdfs:label "bottomDataProperty" .


###  http://www.w3.org/2002/07/owl#cardinality
owl:cardinality rdf:type owl:DatatypeProperty ;
                rdfs:range xsd:nonNegativeInteger ;
                rdfs:comment "The property that determines the cardinality of an exact cardinality restriction." ;
                rdfs:isDefinedBy owl: ;
                rdfs:label "cardinality" .


###  http://www.w3.org/2002/07/owl#maxCardinality
owl:maxCardinality rdf:type owl:DatatypeProperty ;
                   rdfs:range xsd:nonNegativeInteger ;
                   rdfs:comment "The property that determines the cardinality of a maximum cardinality restriction." ;
                   rdfs:isDefinedBy owl: ;
                   rdfs:label "maxCardinality" .


###  http://www.w3.org/2002/07/owl#maxQualifiedCardinality
owl:maxQualifiedCardinality rdf:type owl:DatatypeProperty ;
                            rdfs:range xsd:nonNegativeInteger ;
                            rdfs:comment "The property that determines the cardinality of a maximum qualified cardinality restriction." ;
                            rdfs:isDefinedBy owl: ;
                            rdfs:label "maxQualifiedCardinality" .


###  http://www.w3.org/2002/07/owl#minCardinality
owl:minCardinality rdf:type owl:DatatypeProperty ;
                   rdfs:range xsd:nonNegativeInteger ;
                   rdfs:comment "The property that determines the cardinality of a minimum cardinality restriction." ;
                   rdfs:isDefinedBy owl: ;
                   rdfs:label "minCardinality" .


###  http://www.w3.org/2002/07/owl#minQualifiedCardinality
owl:minQualifiedCardinality rdf:type owl:DatatypeProperty ;
                            rdfs:range xsd:nonNegativeInteger ;
                            rdfs:comment "The property that determines the cardinality of a minimum qualified cardinality restriction." ;
                            rdfs:isDefinedBy owl: ;
                            rdfs:label "minQualifiedCardinality" .


###  http://www.w3.org/2002/07/owl#qualifiedCardinality
owl:qualifiedCardinality rdf:type owl:DatatypeProperty ;
                         rdfs:range xsd:nonNegativeInteger ;
                         rdfs:comment "The property that determines the cardinality of an exact qualified cardinality restriction." ;
                         rdfs:isDefinedBy owl: ;
                         rdfs:label "qualifiedCardinality" .


###  http://www.w3.org/2002/07/owl#topDataProperty
owl:topDataProperty rdf:type owl:DatatypeProperty ;
                    rdfs:domain owl:Thing ;
                    rdfs:range rdfs:Literal ;
                    rdfs:comment "The data property that relates every individual to every data value." ;
                    rdfs:isDefinedBy owl: ;
                    rdfs:label "topDataProperty" .


#################################################################
#    Classes
#################################################################

###  fibo-fbc-fi-fi:NegotiableSecurity
<fibo-fbc-fi-fi:NegotiableSecurity> rdf:type owl:Class ;
                                    rdfs:subClassOf <https://spec.edmcouncil.org/fibo/ontology/FND/Agreements/Contracts/TransferableContract> ;
                                    rdfs:comment "Security that can be transferred to another party"@en ;
                                    rdfs:label "NegotiableSecurity"@en .


###  fibo-fnd-agr-ctr:AssignableContract
<fibo-fnd-agr-ctr:AssignableContract> rdf:type owl:Class ;
                                      rdfs:subClassOf <https://spec.edmcouncil.org/fibo/ontology/FND/Agreements/Contracts/TransferableContract> ;
                                      rdfs:comment "Contract in which contract holder (assignor) may transfer some or all of their rights and obligations to another party (assignee)"@en ;
                                      rdfs:label "AssignableContract"@en .


###  fibo-fnd-agr-ctr:NovateableContract
<fibo-fnd-agr-ctr:NovateableContract> rdf:type owl:Class ;
                                      rdfs:subClassOf <https://spec.edmcouncil.org/fibo/ontology/FND/Agreements/Contracts/TransferableContract> ;
                                      rdfs:comment "Contract that may be replaced by another contract, and in that event, extinguishes the rights and obligations in effect under the original contract with those in the new agreement."@en ;
                                      rdfs:label "NovateableContract"@en .


###  fibo-fnd-plc-adr:Address
<fibo-fnd-plc-adr:Address> rdf:type owl:Class ;
                           rdfs:subClassOf <http://www.w3.org/ns/dpv#Identifying> ;
                           rdfs:comment "Index to a location to which communications may be delivered."@en ;
                           rdfs:label "Address"@en .


###  fibo-fnd-plc-adr:ConventionalStreetAddress
<fibo-fnd-plc-adr:ConventionalStreetAddress> rdf:type owl:Class ;
                                             rdfs:subClassOf <fibo-fnd-plc-adr:PhysicalAddress> ;
                                             rdfs:comment "Physical address that identifies a location on a street to which communications may be delivered."@en ;
                                             rdfs:label "Conventional Street Address"@en .


###  fibo-fnd-plc-adr:PhysicalAddress
<fibo-fnd-plc-adr:PhysicalAddress> rdf:type owl:Class ;
                                   rdfs:subClassOf <fibo-fnd-plc-adr:Address> ;
                                   rdfs:comment "Physical address where communications can be addressed, papers served or representatives located for any kind of organization or person."@en ;
                                   rdfs:label "Physical Address"@en .


###  fibo-fnd-plc-adr:StreetAddress
<fibo-fnd-plc-adr:StreetAddress> rdf:type owl:Class ;
                                 rdfs:subClassOf <fibo-fnd-plc-adr:Address> ;
                                 rdfs:comment "Index to a location that consists of a primary address number, predirectional, street name, suffix, postdirectional, and an optional secondary unit."@en ;
                                 rdfs:label "Street Address"@en .


###  http://mmisw.org/ont/univmemphis/sensor#GPS
<http://mmisw.org/ont/univmemphis/sensor#GPS> rdf:type owl:Class ;
                                              rdfs:subClassOf :Sensor ;
                                              rdfs:comment "A GPS Sensor"@en ;
                                              rdfs:label "GPS"@en .


###  http://mmisw.org/ont/univmemphis/sensor#Humidity
<http://mmisw.org/ont/univmemphis/sensor#Humidity> rdf:type owl:Class ;
                                                   rdfs:subClassOf :Sensor ;
                                                   rdfs:comment "A Humidity Sensor"@en ;
                                                   rdfs:label "Humidity"@en .


###  http://mmisw.org/ont/univmemphis/sensor#Light
<http://mmisw.org/ont/univmemphis/sensor#Light> rdf:type owl:Class ;
                                                rdfs:subClassOf :Sensor ;
                                                rdfs:comment "A Light Sensor"@en ;
                                                rdfs:label "Light"@en .


###  http://mmisw.org/ont/univmemphis/sensor#Motion
<http://mmisw.org/ont/univmemphis/sensor#Motion> rdf:type owl:Class ;
                                                 rdfs:subClassOf :Sensor ;
                                                 rdfs:comment "A Motion Sensor"@en ;
                                                 rdfs:label "Motion"@en .


###  http://mmisw.org/ont/univmemphis/sensor#Non-Imaging
<http://mmisw.org/ont/univmemphis/sensor#Non-Imaging> rdf:type owl:Class ;
                                                      rdfs:subClassOf :Sensor ;
                                                      rdfs:comment "A Non-Imaging Sensor"@en ;
                                                      rdfs:label "Non-Imaging"@en .


###  http://mmisw.org/ont/univmemphis/sensor#Orientation
<http://mmisw.org/ont/univmemphis/sensor#Orientation> rdf:type owl:Class ;
                                                      rdfs:subClassOf :Sensor ;
                                                      rdfs:comment "An Orientation Sensor"@en ;
                                                      rdfs:label "Orientation"@en .


###  http://ontologies.atb-bremen.de/smashHitCore#BuildingData
:BuildingData rdf:type owl:Class ;
              rdfs:subClassOf :SensorDataCategory ;
              rdfs:label "Building Data"@en .


###  http://ontologies.atb-bremen.de/smashHitCore#CarData
:CarData rdf:type owl:Class ;
         rdfs:subClassOf :SensorDataCategory ;
         rdfs:label "Car Data"@en .


###  http://ontologies.atb-bremen.de/smashHitCore#City
:City rdf:type owl:Class ;
      rdfs:subClassOf <http://purl.org/adaptcentre/openscience/ontologies/consent#Location> .


###  http://ontologies.atb-bremen.de/smashHitCore#ConsentID
:ConsentID rdf:type owl:Class ;
           rdfs:subClassOf :consent ,
                           owl:Thing ;
           rdfs:comment "The identifier property represents any kind of identifier for any kind of Thing, such as ISBNs, GTIN codes, UUIDs etc. Schema.org provides dedicated properties for representing many of these, either as textual strings or as URL (URI) links."@en .


###  http://ontologies.atb-bremen.de/smashHitCore#ConsentStatus
:ConsentStatus rdf:type owl:Class ;
               rdfs:subClassOf rdf:Status ;
               rdfs:comment "Specifies the status of consent."@en ;
               rdfs:label "Consent Status"@en .


###  http://ontologies.atb-bremen.de/smashHitCore#ContractId
:ContractId rdf:type owl:Class ;
            rdfs:subClassOf owl:Thing ,
                            <https://spec.edmcouncil.org/fibo/ontology/FND/Agreements/Contracts/Contract_> ;
            rdfs:comment "The identifier property represents any kind of identifier for any kind of Thing, such as ISBNs, GTIN codes, UUIDs etc. Schema.org provides dedicated properties for representing many of these, either as textual strings or as URL (URI) links."@en ;
            rdfs:label "ContractId"@en .


###  http://ontologies.atb-bremen.de/smashHitCore#ContractProvider
:ContractProvider rdf:type owl:Class ;
                  rdfs:subClassOf <http://www.w3.org/ns/dcat#Role> .


###  http://ontologies.atb-bremen.de/smashHitCore#ContractRequester
:ContractRequester rdf:type owl:Class ;
                   rdfs:subClassOf <http://www.w3.org/ns/dcat#Role> .


###  http://ontologies.atb-bremen.de/smashHitCore#Country
:Country rdf:type owl:Class ;
         rdfs:subClassOf <http://purl.org/adaptcentre/openscience/ontologies/consent#Location> .


###  http://ontologies.atb-bremen.de/smashHitCore#DataController
:DataController rdf:type owl:Class ;
                rdfs:subClassOf <http://www.w3.org/ns/dcat#Role> .


###  http://ontologies.atb-bremen.de/smashHitCore#DataOwner
:DataOwner rdf:type owl:Class ;
           rdfs:subClassOf <http://www.w3.org/ns/dcat#Role> .


###  http://ontologies.atb-bremen.de/smashHitCore#DataProtectionOfficer
:DataProtectionOfficer rdf:type owl:Class ;
                       rdfs:subClassOf <http://www.w3.org/ns/dcat#Role> .


###  http://ontologies.atb-bremen.de/smashHitCore#DataProvider
:DataProvider rdf:type owl:Class ;
              rdfs:subClassOf <http://www.w3.org/ns/dcat#Role> .


###  http://ontologies.atb-bremen.de/smashHitCore#DataRequester
:DataRequester rdf:type owl:Class ;
               rdfs:subClassOf <http://www.w3.org/ns/dcat#Role> .


###  http://ontologies.atb-bremen.de/smashHitCore#DataType
:DataType rdf:type owl:Class ;
          rdfs:subClassOf :metadata ;
          rdfs:label "DataType"@en .


###  http://ontologies.atb-bremen.de/smashHitCore#Device
:Device rdf:type owl:Class ;
        rdfs:subClassOf :Source ;
        rdfs:label "Device"@en .


###  http://ontologies.atb-bremen.de/smashHitCore#ExpirationDate
:ExpirationDate rdf:type owl:Class ;
                rdfs:subClassOf <http://purl.org/adaptcentre/openscience/ontologies/consent#Context> .


###  http://ontologies.atb-bremen.de/smashHitCore#Granted
:Granted rdf:type owl:Class ;
         rdfs:subClassOf <https://w3id.org/GConsent#StatusValidForProcessing> .


###  http://ontologies.atb-bremen.de/smashHitCore#Hash
:Hash rdf:type owl:Class ;
      rdfs:subClassOf :metadata ;
      rdfs:comment "A hash function is any function that can be used to map data of arbitrary size to fixed-size values. smashHit uses hashes for traceability."@en .


###  http://ontologies.atb-bremen.de/smashHitCore#Mileage
:Mileage rdf:type owl:Class ;
         rdfs:subClassOf :Sensor .


###  http://ontologies.atb-bremen.de/smashHitCore#PersonalData
:PersonalData rdf:type owl:Class ;
              rdfs:subClassOf <http://www.w3.org/ns/dcat#Resource> ;
              rdfs:label "PersonalData"@en .


###  http://ontologies.atb-bremen.de/smashHitCore#PhysicalLocation
:PhysicalLocation rdf:type owl:Class ;
                  rdfs:subClassOf <http://purl.org/dc/terms/Location> ;
                  rdfs:comment "Spatial location defined by e.g. its GPS coordinates"@en ;
                  rdfs:label "PhysicalLocation"@en .


###  http://ontologies.atb-bremen.de/smashHitCore#Region
:Region rdf:type owl:Class ;
        rdfs:subClassOf <http://purl.org/adaptcentre/openscience/ontologies/consent#Location> .


###  http://ontologies.atb-bremen.de/smashHitCore#Revoked
:Revoked rdf:type owl:Class ;
         rdfs:subClassOf <https://w3id.org/GConsent#StatusInvalidForProcessing> .


###  http://ontologies.atb-bremen.de/smashHitCore#Risk
:Risk rdf:type owl:Class ;
      rdfs:subClassOf owl:Thing ;
      rdfs:comment "Risks associated with the processing of personal data and countermeasures"@en ;
      rdfs:label "Risk"@en .


###  http://ontologies.atb-bremen.de/smashHitCore#Sensor
:Sensor rdf:type owl:Class ;
        rdfs:subClassOf :Device ;
        rdfs:label "Sensor"@en .


###  http://ontologies.atb-bremen.de/smashHitCore#SensorData
:SensorData rdf:type owl:Class ;
            rdfs:subClassOf <http://www.w3.org/ns/dcat#Resource> ;
            rdfs:label "SensorData"@en .


###  http://ontologies.atb-bremen.de/smashHitCore#SensorDataCategory
:SensorDataCategory rdf:type owl:Class ;
                    rdfs:subClassOf owl:Thing ;
                    rdfs:label "SensorDataCategory"@en .


###  http://ontologies.atb-bremen.de/smashHitCore#Source
:Source rdf:type owl:Class ;
        rdfs:subClassOf :metadata ;
        rdfs:label "Source"@en .


###  http://ontologies.atb-bremen.de/smashHitCore#State
:State rdf:type owl:Class ;
       rdfs:subClassOf <http://purl.org/adaptcentre/openscience/ontologies/consent#Location> .


###  http://ontologies.atb-bremen.de/smashHitCore#StorageLocation
:StorageLocation rdf:type owl:Class ;
                 rdfs:subClassOf <http://purl.org/dc/terms/Location> ;
                 rdfs:comment "Technical storage location defined e.g. by a URL"@en ;
                 rdfs:label "StorageLocation"@en .


###  http://ontologies.atb-bremen.de/smashHitCore#TelephoneNumber
:TelephoneNumber rdf:type owl:Class ;
                 rdfs:subClassOf <http://www.w3.org/ns/dpv#Contact> .


###  http://ontologies.atb-bremen.de/smashHitCore#agentid
:agentid rdf:type owl:Class ;
         rdfs:subClassOf <http://www.w3.org/ns/prov#Agent> .


###  http://ontologies.atb-bremen.de/smashHitCore#consent
:consent rdf:type owl:Class ;
         rdfs:subClassOf owl:Thing ;
         rdfs:comment "Consent of the data subject means any freely given, specific, informed and unambiguous indication of the data subject’s wishes by which he or she, by a statement or by a clear affirmative action, signifies agreement to the processing of personal data relating to him or her." ;
         rdfs:label "Consent"@en .


###  http://ontologies.atb-bremen.de/smashHitCore#contract
:contract rdf:type owl:Class .


###  http://ontologies.atb-bremen.de/smashHitCore#dalicc
:dalicc rdf:type owl:Class .


###  http://ontologies.atb-bremen.de/smashHitCore#hasContractStatus
:hasContractStatus rdf:type owl:Class .


###  http://ontologies.atb-bremen.de/smashHitCore#hasEmail
:hasEmail rdf:type owl:Class .


###  http://ontologies.atb-bremen.de/smashHitCore#hasMinimumDuration
:hasMinimumDuration rdf:type owl:Class .


###  http://ontologies.atb-bremen.de/smashHitCore#hasTelephone
:hasTelephone rdf:type owl:Class .


###  http://ontologies.atb-bremen.de/smashHitCore#license
:license rdf:type owl:Class ;
         rdfs:subClassOf owl:Thing .


###  http://ontologies.atb-bremen.de/smashHitCore#metadata
:metadata rdf:type owl:Class ;
          rdfs:subClassOf owl:Thing ;
          rdfs:comment """Metadata summarizes basic information about data, making finding & working with particular instances of data easier.
Some examples of basic metadata are author, date created, date modified, and file size. Metadata is also used for unstructured data such as images, video, web pages, spreadsheets, etc. Web pages often include metadata in the form of meta tags.""" ;
          rdfs:label "Metadata"@en .


###  http://purl.org/adaptcentre/openscience/ontologies/consent#AppBased
<http://purl.org/adaptcentre/openscience/ontologies/consent#AppBased> rdf:type owl:Class ;
                                                                      rdfs:subClassOf <http://purl.org/adaptcentre/openscience/ontologies/consent#ConsentFormat> ;
                                                                      rdfs:comment """It identifies if the consent is taken in the form of mobile application.

It defines if the consent is taken in the form of mobile application."""@en ;
                                                                      rdfs:label "AppBased"@en .


###  http://purl.org/adaptcentre/openscience/ontologies/consent#Audio
<http://purl.org/adaptcentre/openscience/ontologies/consent#Audio> rdf:type owl:Class ;
                                                                   rdfs:subClassOf <http://purl.org/adaptcentre/openscience/ontologies/consent#ConsentFormat> ;
                                                                   rdfs:comment """It is used to identify if the consent is taken in the form of audio.

It identifies if the consent is taken in the form of audio."""@en ;
                                                                   rdfs:label "Audio"@en .


###  http://purl.org/adaptcentre/openscience/ontologies/consent#ConsentFormat
<http://purl.org/adaptcentre/openscience/ontologies/consent#ConsentFormat> rdf:type owl:Class ;
                                                                           rdfs:subClassOf <https://w3id.org/GConsent#Medium> ;
                                                                           rdfs:comment """It is used to record at what format the consent was obtained.

'consent format' defines the format was used to obtain the consent."""@en ;
                                                                           rdfs:label "ConsentFormat"@en .


###  http://purl.org/adaptcentre/openscience/ontologies/consent#Context
<http://purl.org/adaptcentre/openscience/ontologies/consent#Context> rdf:type owl:Class ;
                                                                     rdfs:subClassOf :consent ;
                                                                     rdfs:comment """Context is used to keep track of the contextual information while giving, modifying or revoking consent.

It defines at what context the consent was given."""@en ;
                                                                     rdfs:label "ConsentContext"@en .


###  http://purl.org/adaptcentre/openscience/ontologies/consent#Location
<http://purl.org/adaptcentre/openscience/ontologies/consent#Location> rdf:type owl:Class ;
                                                                      rdfs:subClassOf <http://purl.org/adaptcentre/openscience/ontologies/consent#Context> ;
                                                                      rdfs:comment "The location where consent was given/revoked."@en ;
                                                                      rdfs:label "ConsentGivenAtLocation"@en .


###  http://purl.org/adaptcentre/openscience/ontologies/consent#OnlineForm
<http://purl.org/adaptcentre/openscience/ontologies/consent#OnlineForm> rdf:type owl:Class ;
                                                                        rdfs:subClassOf <http://purl.org/adaptcentre/openscience/ontologies/consent#ConsentFormat> ;
                                                                        rdfs:comment """It identifies if the consent is taken in the form of an online form.
"""@en ;
                                                                        rdfs:label "OnlineForm"@en .


###  http://purl.org/adaptcentre/openscience/ontologies/consent#OnlineOptInOption
<http://purl.org/adaptcentre/openscience/ontologies/consent#OnlineOptInOption> rdf:type owl:Class ;
                                                                               rdfs:subClassOf <http://purl.org/adaptcentre/openscience/ontologies/consent#ConsentFormat> ;
                                                                               rdfs:comment """It identifies if the consent is taken as an online opt-in option.
"""@en ;
                                                                               rdfs:label "Opt-InOption"@en .


###  http://purl.org/adaptcentre/openscience/ontologies/consent#Paper
<http://purl.org/adaptcentre/openscience/ontologies/consent#Paper> rdf:type owl:Class ;
                                                                   rdfs:subClassOf <http://purl.org/adaptcentre/openscience/ontologies/consent#ConsentFormat> ;
                                                                   rdfs:comment """It identifies if the consent is taken on paper.
"""@en ;
                                                                   rdfs:label "Paper"@en .


###  http://purl.org/adaptcentre/openscience/ontologies/consent#Time
<http://purl.org/adaptcentre/openscience/ontologies/consent#Time> rdf:type owl:Class ;
                                                                  rdfs:subClassOf <http://purl.org/adaptcentre/openscience/ontologies/consent#Context> ;
                                                                  rdfs:comment "The time when consent was given/revoked."@en ;
                                                                  rdfs:label "ConsentTime"@en .


###  http://purl.org/adaptcentre/openscience/ontologies/consent#Video
<http://purl.org/adaptcentre/openscience/ontologies/consent#Video> rdf:type owl:Class ;
                                                                   rdfs:subClassOf <http://purl.org/adaptcentre/openscience/ontologies/consent#ConsentFormat> ;
                                                                   rdfs:comment """It identifies if the consent is taken in the form of video.
"""@en ;
                                                                   rdfs:label "Video"@en .


###  http://purl.org/dc/terms/Location
<http://purl.org/dc/terms/Location> rdf:type owl:Class ;
                                    rdfs:subClassOf :metadata ;
                                    rdfs:comment "A spatial region or named place."@en ;
                                    rdfs:label "Location"@en .


###  http://purl.org/dc/terms/PeriodOfTime
<http://purl.org/dc/terms/PeriodOfTime> rdf:type owl:Class ;
                                        rdfs:subClassOf :metadata ;
                                        rdfs:comment "An interval of time that is named or defined by its start and end."@en ;
                                        rdfs:label "Period of Time"@en .


###  http://www.w3.org/1999/02/22-rdf-syntax-ns#Data_Processing
rdf:Data_Processing rdf:type owl:Class ;
                    rdfs:comment """Processing is defined by the GDPR (Article 4-2) as \"any operation or set of operations which is performed on personal data or on sets of personal data, whether or not by automated means, such as collection, recording, organisation, structuring, storage, adaptation or alteration, retrieval, consultation, use, disclosure by transmission, dissemination or otherwise making available, alignment or combination, restriction, erasure or destruction;\".

Processing can be considered as the action, within an activity for example, that uses data in a particular or specific way. Therefore, processing specifies what is happening to/with the data.""" ;
                    rdfs:label "DataProcessing"@en .


###  http://www.w3.org/1999/02/22-rdf-syntax-ns#Status
rdf:Status rdf:type owl:Class ;
           rdfs:comment """Describes the status of consent. 
.
.
Status of contracts to be added later."""@en ;
           rdfs:label "Status"@en .


###  http://www.w3.org/2002/07/owl#Thing
owl:Thing rdf:type owl:Class ;
          rdfs:comment "The class of OWL individuals." ;
          rdfs:isDefinedBy owl: ;
          rdfs:label "Thing" .


###  http://www.w3.org/2004/02/skos/core#Concept
<http://www.w3.org/2004/02/skos/core#Concept> rdf:type owl:Class ;
                                              rdfs:subClassOf owl:Thing ;
                                              rdfs:comment "An idea or notion; a unit of thought."@en ;
                                              rdfs:label "Concept"@en .


###  http://www.w3.org/ns/dcat#Dataset
<http://www.w3.org/ns/dcat#Dataset> rdf:type owl:Class ;
                                    rdfs:subClassOf <http://www.w3.org/ns/dcat#Resource> ;
                                    rdfs:comment "A collection of data, published or curated by a single agent, and available for access or download in one or more representations."@en ;
                                    rdfs:label "Dataset"@en .


###  http://www.w3.org/ns/dcat#Resource
<http://www.w3.org/ns/dcat#Resource> rdf:type owl:Class ;
                                     rdfs:subClassOf owl:Thing ;
                                     rdfs:comment "Resource published or curated by a single agent."@en ;
                                     rdfs:label "Resource"@en .


###  http://www.w3.org/ns/dcat#Role
<http://www.w3.org/ns/dcat#Role> rdf:type owl:Class ;
                                 rdfs:subClassOf <http://www.w3.org/2004/02/skos/core#Concept> ;
                                 rdfs:comment "A role is the function of a resource or agent with respect to another resource, in the context of resource attribution or resource relationships."@en ;
                                 rdfs:label "Role"@en .


###  http://www.w3.org/ns/dcat#endDate
<http://www.w3.org/ns/dcat#endDate> rdf:type owl:Class .


###  http://www.w3.org/ns/dcat#startDate
<http://www.w3.org/ns/dcat#startDate> rdf:type owl:Class .


###  http://www.w3.org/ns/dpv#AcademicResearch
<http://www.w3.org/ns/dpv#AcademicResearch> rdf:type owl:Class ;
                                            rdfs:subClassOf <http://www.w3.org/ns/dpv#ResearchAndDevelopment> ;
                                            rdfs:comment "Research conducted in an academic context e.g. within universities"@en ;
                                            rdfs:label "Academic Research"@en .


###  http://www.w3.org/ns/dpv#AccessControl
<http://www.w3.org/ns/dpv#AccessControl> rdf:type owl:Class ;
                                         rdfs:subClassOf <http://www.w3.org/ns/dpv#Security> ;
                                         rdfs:comment "To conduct or enforce access control"@en ;
                                         rdfs:label "Access Control"@en .


###  http://www.w3.org/ns/dpv#Adapt
<http://www.w3.org/ns/dpv#Adapt> rdf:type owl:Class ;
                                 rdfs:subClassOf rdf:Data_Processing ;
                                 rdfs:comment "to modify the data, often rewritten into a new form for a new use"@en ;
                                 rdfs:label "Adapt"@en .


###  http://www.w3.org/ns/dpv#Align
<http://www.w3.org/ns/dpv#Align> rdf:type owl:Class ;
                                 rdfs:subClassOf rdf:Data_Processing ;
                                 rdfs:comment "to adjust the data to be in relation to another data"@en ;
                                 rdfs:label "Align"@en .


###  http://www.w3.org/ns/dpv#Alter
<http://www.w3.org/ns/dpv#Alter> rdf:type owl:Class ;
                                 rdfs:subClassOf rdf:Data_Processing ;
                                 rdfs:comment "to change the data withouth changing it into something else"@en ;
                                 rdfs:label "Alter"@en .


###  http://www.w3.org/ns/dpv#Authenticating
<http://www.w3.org/ns/dpv#Authenticating> rdf:type owl:Class ;
                                          rdfs:subClassOf <http://www.w3.org/ns/dpv#Internal> ;
                                          rdfs:comment "Information used to authenticate an individual with something they know"@en ;
                                          rdfs:label "Authenticating"@en .


###  http://www.w3.org/ns/dpv#Collect
<http://www.w3.org/ns/dpv#Collect> rdf:type owl:Class ;
                                   rdfs:subClassOf rdf:Data_Processing ;
                                   rdfs:comment "to gather data from someone"@en ;
                                   rdfs:label "Collect"@en .


###  http://www.w3.org/ns/dpv#Combine
<http://www.w3.org/ns/dpv#Combine> rdf:type owl:Class ;
                                   rdfs:subClassOf rdf:Data_Processing ;
                                   rdfs:comment "to join or merge data"@en ;
                                   rdfs:label "Combine"@en .


###  http://www.w3.org/ns/dpv#CommercialInterest
<http://www.w3.org/ns/dpv#CommercialInterest> rdf:type owl:Class ;
                                              rdfs:subClassOf <http://www.w3.org/ns/dpv#Purpose> ;
                                              rdfs:comment "For purposes of commercial activities i.e. of profit or benefit to the Controller"@en ;
                                              rdfs:label "Commercial Interest"@en .


###  http://www.w3.org/ns/dpv#CommercialResearch
<http://www.w3.org/ns/dpv#CommercialResearch> rdf:type owl:Class ;
                                              rdfs:subClassOf <http://www.w3.org/ns/dpv#ResearchAndDevelopment> ;
                                              rdfs:comment "Research conducted in a commercial setting e.g. in a company"@en ;
                                              rdfs:label "Commercial Research"@en .


###  http://www.w3.org/ns/dpv#Consult
<http://www.w3.org/ns/dpv#Consult> rdf:type owl:Class ;
                                   rdfs:subClassOf rdf:Data_Processing ;
                                   rdfs:comment "to consult or query data"@en ;
                                   rdfs:label "Consult"@en .


###  http://www.w3.org/ns/dpv#Contact
<http://www.w3.org/ns/dpv#Contact> rdf:type owl:Class ;
                                   rdfs:subClassOf <http://www.w3.org/ns/dpv#Tracking> ;
                                   rdfs:comment "Information that can be used for contacting an individual e.g. email address or phone number"@en ;
                                   rdfs:label "Contact"@en .


###  http://www.w3.org/ns/dpv#CreateEventRecommendations
<http://www.w3.org/ns/dpv#CreateEventRecommendations> rdf:type owl:Class ;
                                                      rdfs:subClassOf <http://www.w3.org/ns/dpv#CreatePersonalizedRecommendations> ;
                                                      rdfs:comment "Create and provide personalised recommendations for events to the individual"@en ;
                                                      rdfs:label "Create Event Recommendations"@en .


###  http://www.w3.org/ns/dpv#CreatePersonalizedRecommendations
<http://www.w3.org/ns/dpv#CreatePersonalizedRecommendations> rdf:type owl:Class ;
                                                             rdfs:subClassOf <http://www.w3.org/ns/dpv#ServicePersonalization> ;
                                                             rdfs:comment "Create and provide personalised recommendations to the individual"@en ;
                                                             rdfs:label "Create Personalized Recommendations"@en .


###  http://www.w3.org/ns/dpv#CreateProductRecommendations
<http://www.w3.org/ns/dpv#CreateProductRecommendations> rdf:type owl:Class ;
                                                        rdfs:subClassOf <http://www.w3.org/ns/dpv#CreatePersonalizedRecommendations> ;
                                                        rdfs:comment "To create product recommendations e.g. suggest similar products"@en ;
                                                        rdfs:label "Create Product Recommendations"@en .


###  http://www.w3.org/ns/dpv#CustomerCare
<http://www.w3.org/ns/dpv#CustomerCare> rdf:type owl:Class ;
                                        rdfs:subClassOf <http://www.w3.org/ns/dpv#ServiceProvision> ;
                                        rdfs:comment "Processes related to providing assistance for customer satisfaction"@en ;
                                        rdfs:label "Customer Care"@en .


###  http://www.w3.org/ns/dpv#DeliveryOfGoods
<http://www.w3.org/ns/dpv#DeliveryOfGoods> rdf:type owl:Class ;
                                           rdfs:subClassOf <http://www.w3.org/ns/dpv#ServiceProvision> ;
                                           rdfs:comment "To deliver goods and services"@en ;
                                           rdfs:label "Delivery of Goods"@en .


###  http://www.w3.org/ns/dpv#Destruct
<http://www.w3.org/ns/dpv#Destruct> rdf:type owl:Class ;
                                    rdfs:subClassOf rdf:Data_Processing ;
                                    rdfs:comment "to process data in a way it no longer exists or cannot be repaired"@en ;
                                    rdfs:label "Destruct"@en .


###  http://www.w3.org/ns/dpv#DiscloseByTransmission
<http://www.w3.org/ns/dpv#DiscloseByTransmission> rdf:type owl:Class ;
                                                  rdfs:subClassOf rdf:Data_Processing ;
                                                  rdfs:comment "to disclose data by means of transmission"@en ;
                                                  rdfs:label "Disclose by Transmission"@en .


###  http://www.w3.org/ns/dpv#Disseminate
<http://www.w3.org/ns/dpv#Disseminate> rdf:type owl:Class ;
                                       rdfs:subClassOf rdf:Data_Processing ;
                                       rdfs:comment "to spread data throughout"@en ;
                                       rdfs:label "Disseminate"@en .


###  http://www.w3.org/ns/dpv#EmailAddress
<http://www.w3.org/ns/dpv#EmailAddress> rdf:type owl:Class ;
                                        rdfs:subClassOf <http://www.w3.org/ns/dpv#Contact> ;
                                        rdfs:comment "Information about an individual's Email address."@en ;
                                        rdfs:label "EmailAddress"@en .


###  http://www.w3.org/ns/dpv#Erase
<http://www.w3.org/ns/dpv#Erase> rdf:type owl:Class ;
                                 rdfs:subClassOf rdf:Data_Processing ;
                                 rdfs:comment "to delete data"@en ;
                                 rdfs:label "Erase"@en .


###  http://www.w3.org/ns/dpv#External
<http://www.w3.org/ns/dpv#External> rdf:type owl:Class ;
                                    rdfs:subClassOf <http://www.w3.org/ns/dpv#PersonalDataCategory> ;
                                    rdfs:comment "Personal Data that can be observed by another person i.e. has external characteristics that make it visible"@en ;
                                    rdfs:label "External"@en .


###  http://www.w3.org/ns/dpv#Financial
<http://www.w3.org/ns/dpv#Financial> rdf:type owl:Class ;
                                     rdfs:subClassOf <http://www.w3.org/ns/dpv#PersonalDataCategory> ;
                                     rdfs:comment "Personal data regarding finance or monetary information"@en ;
                                     rdfs:label "Financial"@en .


###  http://www.w3.org/ns/dpv#FraudPreventionAndDetection
<http://www.w3.org/ns/dpv#FraudPreventionAndDetection> rdf:type owl:Class ;
                                                       rdfs:subClassOf <http://www.w3.org/ns/dpv#Security> ;
                                                       rdfs:comment "To detect and prevent fraud"@en ;
                                                       rdfs:label "Fraud Prevention and Detection"@en .


###  http://www.w3.org/ns/dpv#Identifying
<http://www.w3.org/ns/dpv#Identifying> rdf:type owl:Class ;
                                       rdfs:subClassOf <http://www.w3.org/ns/dpv#External> ;
                                       rdfs:comment "Information that uniquely or semi-uniquely identifies a specific individual"@en ;
                                       rdfs:label "Identifying"@en .


###  http://www.w3.org/ns/dpv#IdentityVerification
<http://www.w3.org/ns/dpv#IdentityVerification> rdf:type owl:Class ;
                                                rdfs:subClassOf <http://www.w3.org/ns/dpv#Security> ;
                                                rdfs:comment "To verify and authorise identity"@en ;
                                                rdfs:label "Identity Verification"@en .


###  http://www.w3.org/ns/dpv#ImproveExistingProductsAndServices
<http://www.w3.org/ns/dpv#ImproveExistingProductsAndServices> rdf:type owl:Class ;
                                                              rdfs:subClassOf <http://www.w3.org/ns/dpv#OptimisationForController> ;
                                                              rdfs:comment "To improve existing products and services"@en ;
                                                              rdfs:label "Improve Existing Products and Services"@en .


###  http://www.w3.org/ns/dpv#ImproveInternalCRMProcesses
<http://www.w3.org/ns/dpv#ImproveInternalCRMProcesses> rdf:type owl:Class ;
                                                       rdfs:subClassOf <http://www.w3.org/ns/dpv#OptimisationForController> ;
                                                       rdfs:comment "To improve customer-relationship management (CRM) processes"@en ;
                                                       rdfs:label "Improve Internal CRM Processes"@en .


###  http://www.w3.org/ns/dpv#IncreaseServiceRobustness
<http://www.w3.org/ns/dpv#IncreaseServiceRobustness> rdf:type owl:Class ;
                                                     rdfs:subClassOf <http://www.w3.org/ns/dpv#OptimisationForController> ;
                                                     rdfs:comment "To improve the robustness and resilience of services"@en ;
                                                     rdfs:label "Increase Service Robustness"@en .


###  http://www.w3.org/ns/dpv#Internal
<http://www.w3.org/ns/dpv#Internal> rdf:type owl:Class ;
                                    rdfs:subClassOf <http://www.w3.org/ns/dpv#PersonalDataCategory> ;
                                    rdfs:comment "Personal data about characteristics of an individual that are internal i.e. cannot be seen or observed"@en ;
                                    rdfs:label "Internal"@en .


###  http://www.w3.org/ns/dpv#InternalResourceOptimisation
<http://www.w3.org/ns/dpv#InternalResourceOptimisation> rdf:type owl:Class ;
                                                        rdfs:subClassOf <http://www.w3.org/ns/dpv#OptimisationForController> ;
                                                        rdfs:comment "Optimisation of internal resources used by the organisation e.g. resource usage"@en ;
                                                        rdfs:label "Internal Resource Optimisation"@en .


###  http://www.w3.org/ns/dpv#Location
<http://www.w3.org/ns/dpv#Location> rdf:type owl:Class ;
                                    rdfs:subClassOf <http://www.w3.org/ns/dpv#Tracking> ;
                                    rdfs:comment "Information about an individual’s location"@en ;
                                    rdfs:label "Location"@en .


###  http://www.w3.org/ns/dpv#Name
<http://www.w3.org/ns/dpv#Name> rdf:type owl:Class ;
                                owl:equivalentClass <http://www.w3.org/ns/prov#Person> ;
                                rdfs:subClassOf <http://www.w3.org/ns/dpv#Identifying> ;
                                rdfs:comment "A name associated with an individual e.g. given name, nickname."@en ;
                                rdfs:label "Name"@en .


###  http://www.w3.org/ns/dpv#NonCommercialResearch
<http://www.w3.org/ns/dpv#NonCommercialResearch> rdf:type owl:Class ;
                                                 rdfs:subClassOf <http://www.w3.org/ns/dpv#ResearchAndDevelopment> ;
                                                 rdfs:comment "Research conducted in a non-commercial setting e.g. for a non-profit-organisation (NGO)"@en ;
                                                 rdfs:label "Non-Commercial Research"@en .


###  http://www.w3.org/ns/dpv#OfficialID
<http://www.w3.org/ns/dpv#OfficialID> rdf:type owl:Class ;
                                      rdfs:subClassOf <http://www.w3.org/ns/dpv#Identifying> ;
                                      rdfs:comment "Information on an official identification document used by an individual."@en ;
                                      rdfs:label "OfficialID"@en .


###  http://www.w3.org/ns/dpv#OptimisationForConsumer
<http://www.w3.org/ns/dpv#OptimisationForConsumer> rdf:type owl:Class ;
                                                   rdfs:subClassOf <http://www.w3.org/ns/dpv#ServiceOptimization> ;
                                                   rdfs:label "Optimisation for Consumer"@en .


###  http://www.w3.org/ns/dpv#OptimisationForController
<http://www.w3.org/ns/dpv#OptimisationForController> rdf:type owl:Class ;
                                                     rdfs:subClassOf <http://www.w3.org/ns/dpv#ServiceOptimization> ;
                                                     rdfs:label "Optimisation for Controller"@en .


###  http://www.w3.org/ns/dpv#OptimiseUserInterface
<http://www.w3.org/ns/dpv#OptimiseUserInterface> rdf:type owl:Class ;
                                                 rdfs:subClassOf <http://www.w3.org/ns/dpv#OptimisationForConsumer> ;
                                                 rdfs:label "Optimise User Interface"@en .


###  http://www.w3.org/ns/dpv#Organise
<http://www.w3.org/ns/dpv#Organise> rdf:type owl:Class ;
                                    rdfs:subClassOf rdf:Data_Processing ;
                                    rdfs:comment "to organize data for arranging or classifying"@en ;
                                    rdfs:label "Organise"@en .


###  http://www.w3.org/ns/dpv#Ownership
<http://www.w3.org/ns/dpv#Ownership> rdf:type owl:Class ;
                                     rdfs:subClassOf <http://www.w3.org/ns/dpv#Financial> ;
                                     rdfs:comment "Information about things an individual has owned, rented, borrowed, possessed"@en ;
                                     rdfs:label "Ownership"@en .


###  http://www.w3.org/ns/dpv#Password
<http://www.w3.org/ns/dpv#Password> rdf:type owl:Class ;
                                    rdfs:subClassOf <http://www.w3.org/ns/dpv#Authenticating> ;
                                    rdfs:comment "An individual's password used in the process of authenticating the individual as a user accessing a system."@en ;
                                    rdfs:label "Password"@en .


###  http://www.w3.org/ns/dpv#PersonalDataCategory
<http://www.w3.org/ns/dpv#PersonalDataCategory> rdf:type owl:Class ;
                                                rdfs:subClassOf owl:Thing ;
                                                rdfs:comment "A category of personal data (as defined by GDPR article 4.1) from the personal data categories taxonomy, i.e. for instance denoting the category of an object/field or data item that is used for processing"@en ;
                                                rdfs:label "PersonalDataCategory"@en .


###  http://www.w3.org/ns/dpv#PersonalisedBenefits
<http://www.w3.org/ns/dpv#PersonalisedBenefits> rdf:type owl:Class ;
                                                rdfs:subClassOf <http://www.w3.org/ns/dpv#ServicePersonalization> ;
                                                rdfs:comment "Personalisation of benefits received by the user"@en ;
                                                rdfs:label "Personalised Benefits"@en .


###  http://www.w3.org/ns/dpv#Preference
<http://www.w3.org/ns/dpv#Preference> rdf:type owl:Class ;
                                      rdfs:subClassOf <http://www.w3.org/ns/dpv#Internal> ;
                                      rdfs:comment "Information about an individual’s preferences or interests"@en ;
                                      rdfs:label "Preference"@en .


###  http://www.w3.org/ns/dpv#PrivacyPreference
<http://www.w3.org/ns/dpv#PrivacyPreference> rdf:type owl:Class ;
                                             rdfs:subClassOf <http://www.w3.org/ns/dpv#Preference> ;
                                             rdfs:comment "Information about an individual's privacy preferences"@en ;
                                             rdfs:label "PrivacyPreference"@en .


###  http://www.w3.org/ns/dpv#Purpose
<http://www.w3.org/ns/dpv#Purpose> rdf:type owl:Class ;
                                   rdfs:subClassOf owl:Thing ;
                                   rdfs:comment "The purpose of Data Handling, from the purposes Taxonomy"@en ;
                                   rdfs:label "Purpose"@en .


###  http://www.w3.org/ns/dpv#Record
<http://www.w3.org/ns/dpv#Record> rdf:type owl:Class ;
                                  rdfs:subClassOf rdf:Data_Processing ;
                                  rdfs:comment "to make a record (especially media)"@en ;
                                  rdfs:label "Record"@en .


###  http://www.w3.org/ns/dpv#ResearchAndDevelopment
<http://www.w3.org/ns/dpv#ResearchAndDevelopment> rdf:type owl:Class ;
                                                  rdfs:subClassOf <http://www.w3.org/ns/dpv#Purpose> ;
                                                  rdfs:comment "Performing research and developing new methods,products, or services"@en ;
                                                  rdfs:label "Research and Development"@en .


###  http://www.w3.org/ns/dpv#Restrict
<http://www.w3.org/ns/dpv#Restrict> rdf:type owl:Class ;
                                    rdfs:subClassOf rdf:Data_Processing ;
                                    rdfs:comment "to apply a restriction on the processsing of specific records"@en ;
                                    rdfs:label "Restrict"@en .


###  http://www.w3.org/ns/dpv#Retrieve
<http://www.w3.org/ns/dpv#Retrieve> rdf:type owl:Class ;
                                    rdfs:subClassOf rdf:Data_Processing ;
                                    rdfs:comment "to retrieve data, often in an automated manner"@en ;
                                    rdfs:label "Retrieve"@en .


###  http://www.w3.org/ns/dpv#Security
<http://www.w3.org/ns/dpv#Security> rdf:type owl:Class ;
                                    rdfs:subClassOf <http://www.w3.org/ns/dpv#Purpose> ;
                                    rdfs:comment "Security of data"@en ;
                                    rdfs:label "Security"@en .


###  http://www.w3.org/ns/dpv#SellDataToThirdParties
<http://www.w3.org/ns/dpv#SellDataToThirdParties> rdf:type owl:Class ;
                                                  rdfs:subClassOf <http://www.w3.org/ns/dpv#CommercialInterest> ;
                                                  rdfs:comment "To sell data or information to third parties"@en ;
                                                  rdfs:label "Sell Data to Third Parties"@en .


###  http://www.w3.org/ns/dpv#SellInsightsFromData
<http://www.w3.org/ns/dpv#SellInsightsFromData> rdf:type owl:Class ;
                                                rdfs:subClassOf <http://www.w3.org/ns/dpv#CommercialInterest> ;
                                                rdfs:comment "To sell or commercially provide insights obtained from analysis of data"@en ;
                                                rdfs:label "Sell Insights from Data"@en .


###  http://www.w3.org/ns/dpv#SellProductsToDataSubject
<http://www.w3.org/ns/dpv#SellProductsToDataSubject> rdf:type owl:Class ;
                                                     rdfs:subClassOf <http://www.w3.org/ns/dpv#CommercialInterest> ;
                                                     rdfs:comment "To sell products or services to the data subject or user"@en ;
                                                     rdfs:label "Sell Products to Data Subject"@en .


###  http://www.w3.org/ns/dpv#SellTargettedAdvertisements
<http://www.w3.org/ns/dpv#SellTargettedAdvertisements> rdf:type owl:Class ;
                                                       rdfs:subClassOf <http://www.w3.org/ns/dpv#CommercialInterest> ;
                                                       rdfs:comment "To sell or provide targetted advertisements about the user to Third Parties"@en ;
                                                       rdfs:label "Sell Targetted Advertisements"@en .


###  http://www.w3.org/ns/dpv#ServiceOptimization
<http://www.w3.org/ns/dpv#ServiceOptimization> rdf:type owl:Class ;
                                               rdfs:subClassOf <http://www.w3.org/ns/dpv#Purpose> ;
                                               rdfs:label "Service Optimization"@en .


###  http://www.w3.org/ns/dpv#ServicePersonalization
<http://www.w3.org/ns/dpv#ServicePersonalization> rdf:type owl:Class ;
                                                  rdfs:subClassOf <http://www.w3.org/ns/dpv#Purpose> ;
                                                  rdfs:comment "Personalization of service or activity for the user"@en ;
                                                  rdfs:label "Service Personalization"@en .


###  http://www.w3.org/ns/dpv#ServiceProvision
<http://www.w3.org/ns/dpv#ServiceProvision> rdf:type owl:Class ;
                                            rdfs:subClassOf <http://www.w3.org/ns/dpv#Purpose> ;
                                            rdfs:comment "Provision of service or activity"@en ;
                                            rdfs:label "Service Provision"@en .


###  http://www.w3.org/ns/dpv#Share
<http://www.w3.org/ns/dpv#Share> rdf:type owl:Class ;
                                 rdfs:subClassOf rdf:Data_Processing ;
                                 rdfs:comment "to give data (or a portion of it) to others"@en ;
                                 rdfs:label "Share"@en .


###  http://www.w3.org/ns/dpv#Store
<http://www.w3.org/ns/dpv#Store> rdf:type owl:Class ;
                                 rdfs:subClassOf rdf:Data_Processing ;
                                 rdfs:comment "to keep data for future use"@en ;
                                 rdfs:label "Store"@en .


###  http://www.w3.org/ns/dpv#Structure
<http://www.w3.org/ns/dpv#Structure> rdf:type owl:Class ;
                                     rdfs:subClassOf rdf:Data_Processing ;
                                     rdfs:comment "to arrange data according to a structure"@en ;
                                     rdfs:label "Structure"@en .


###  http://www.w3.org/ns/dpv#Tracking
<http://www.w3.org/ns/dpv#Tracking> rdf:type owl:Class ;
                                    rdfs:subClassOf <http://www.w3.org/ns/dpv#PersonalDataCategory> ;
                                    rdfs:comment "Personal data that can be used to track an individual or used as an identifier e.g. location or email"@en ;
                                    rdfs:label "Tracking"@en .


###  http://www.w3.org/ns/dpv#UID
<http://www.w3.org/ns/dpv#UID> rdf:type owl:Class ;
                               rdfs:subClassOf <http://www.w3.org/ns/dpv#Identifying> ;
                               rdfs:comment "An unique identifier used to identify an individual."@en ;
                               rdfs:label "UID"@en .


###  http://www.w3.org/ns/dpv#Use
<http://www.w3.org/ns/dpv#Use> rdf:type owl:Class ;
                               rdfs:subClassOf rdf:Data_Processing ;
                               rdfs:comment "to use data"@en ;
                               rdfs:label "Use"@en .


###  http://www.w3.org/ns/dpv#UserInterfacePersonalisation
<http://www.w3.org/ns/dpv#UserInterfacePersonalisation> rdf:type owl:Class ;
                                                        rdfs:subClassOf <http://www.w3.org/ns/dpv#ServicePersonalization> ;
                                                        rdfs:comment "Personalisation of interfaces presented to the user"@en ;
                                                        rdfs:label "User Interface Personalisation"@en .


###  http://www.w3.org/ns/dpv#Username
<http://www.w3.org/ns/dpv#Username> rdf:type owl:Class ;
                                    rdfs:subClassOf <http://www.w3.org/ns/dpv#Identifying> ;
                                    rdfs:comment "A username used to identify an individual."@en ;
                                    rdfs:label "Username"@en .


###  http://www.w3.org/ns/odrl/2/Asset
<http://www.w3.org/ns/odrl/2/Asset> rdf:type owl:Class ;
                                    rdfs:subClassOf :license ;
                                    rdfs:comment "The Asset entity can be any form of identifiable resource, such as data/information, content/media, applications, or services. Furthermore, it can be used to represent other Asset entities that are needed to undertake the Policy expression, such as with the Duty entity. To describe more details about the Asset, it is recommended to use Dublin Core [dcterms] elements or other content metadata."@en ;
                                    rdfs:label "Asset"@en .


###  http://www.w3.org/ns/odrl/2/AssetCollection
<http://www.w3.org/ns/odrl/2/AssetCollection> rdf:type owl:Class ;
                                              rdfs:subClassOf <http://www.w3.org/ns/odrl/2/Asset> ;
                                              rdfs:comment "An Asset that is collection of individual resources"@en ;
                                              rdfs:label "Asset Collection"@en .


###  http://www.w3.org/ns/odrl/2/Duty
<http://www.w3.org/ns/odrl/2/Duty> rdf:type owl:Class ;
                                   rdfs:subClassOf <http://www.w3.org/ns/odrl/2/Rule> ;
                                   rdfs:comment "The obligation to perform an Action"@en ;
                                   rdfs:label "Duty"@en .


###  http://www.w3.org/ns/odrl/2/Permission
<http://www.w3.org/ns/odrl/2/Permission> rdf:type owl:Class ;
                                         rdfs:subClassOf <http://www.w3.org/ns/odrl/2/Rule> ;
                                         rdfs:comment "The ability to perform an Action over an Asset."@en ;
                                         rdfs:label "Permission"@en .


###  http://www.w3.org/ns/odrl/2/Policy
<http://www.w3.org/ns/odrl/2/Policy> rdf:type owl:Class ;
                                     rdfs:subClassOf :license ;
                                     rdfs:comment "\"A non-empty group of Permissions and/or Prohibitions.\""@en .


###  http://www.w3.org/ns/odrl/2/Rule
<http://www.w3.org/ns/odrl/2/Rule> rdf:type owl:Class ;
                                   rdfs:subClassOf :license ;
                                   rdfs:comment "An abstract concept that represents the common characteristics of Permissions, Prohibitions, and Duties."@en ;
                                   rdfs:label "Rule"@en .


###  http://www.w3.org/ns/odrl/2/Set
<http://www.w3.org/ns/odrl/2/Set> rdf:type owl:Class ;
                                  rdfs:subClassOf <http://www.w3.org/ns/odrl/2/Policy> ;
                                  rdfs:comment """A Policy that expresses a Rule over an Asset.
A Set Policy MUST contain a target Asset, and at least one Rule. A Set Policy is the default Policy subclass. The Set is aimed at scenarios where there is an open criteria for the semantics of the policy expressions and typically refined by other systems/profiles that process the information at a later time. No privileges are granted to any Party (if defined)."""@en ;
                                  rdfs:label "Set"@en .


###  http://www.w3.org/ns/prov#Agent
<http://www.w3.org/ns/prov#Agent> rdf:type owl:Class ;
                                  rdfs:subClassOf owl:Thing ;
                                  rdfs:comment "An agent is something that bears some form of responsibility for an activity taking place, for the existence of an entity, or for another agent's activity. "@en ;
                                  rdfs:label "Agent"@en .


###  http://www.w3.org/ns/prov#Organization
<http://www.w3.org/ns/prov#Organization> rdf:type owl:Class ;
                                         rdfs:subClassOf <http://www.w3.org/ns/prov#Agent> ;
                                         rdfs:comment "An organization is a social or legal institution such as a company, society, etc."@en ;
                                         rdfs:label "Organization"@en .


###  http://www.w3.org/ns/prov#Person
<http://www.w3.org/ns/prov#Person> rdf:type owl:Class ;
                                   rdfs:subClassOf <http://www.w3.org/ns/prov#Agent> ;
                                   rdfs:comment "Person agents are people."@en ;
                                   rdfs:label "Person"@en .


###  http://www.w3.org/ns/prov#SoftwareAgent
<http://www.w3.org/ns/prov#SoftwareAgent> rdf:type owl:Class ;
                                          rdfs:subClassOf <http://www.w3.org/ns/prov#Agent> ;
                                          rdfs:comment "A software agent is running software."@en ;
                                          rdfs:label "SoftwareAgent"@en .


###  https://schema.org/birthDate
<https://schema.org/birthDate> rdf:type owl:Class ;
                               rdfs:subClassOf <http://www.w3.org/ns/dpv#Identifying> ;
                               rdfs:comment "Date of birth"@en ;
                               rdfs:label "birthDate"@en .


###  https://spec.edmcouncil.org/fibo/ontology/DER/DerivativesContracts/DerivativesMasterAgreements/CreditSupportAgreement
<https://spec.edmcouncil.org/fibo/ontology/DER/DerivativesContracts/DerivativesMasterAgreements/CreditSupportAgreement> rdf:type owl:Class ;
                                                                                                                        rdfs:subClassOf <https://spec.edmcouncil.org/fibo/ontology/FND/Agreements/Contracts/Contract_> ;
                                                                                                                        rdfs:comment "Credit support agreement is a kind of contract. (i) Credit support agreement has some beneficiary that is credit support beneficiary. (ii) Credit support agreement is provided by some contract principal."@en ;
                                                                                                                        rdfs:label "CreditSupportAgreement"@en .


###  https://spec.edmcouncil.org/fibo/ontology/FBC/DebtAndEquities/Debt/CreditAgreement
<https://spec.edmcouncil.org/fibo/ontology/FBC/DebtAndEquities/Debt/CreditAgreement> rdf:type owl:Class ;
                                                                                     rdfs:subClassOf <https://spec.edmcouncil.org/fibo/ontology/FND/Agreements/Contracts/Contract_> ;
                                                                                     rdfs:comment "a contractual agreement in which a debtor receives something of value and agrees to repay the creditor at some date in the future, in some form (e.g., cash, securities, etc.), generally with interest"@en ;
                                                                                     rdfs:label "CreditAgreement"@en .


###  https://spec.edmcouncil.org/fibo/ontology/FND/Agreements/Contracts/ContractDocument
<https://spec.edmcouncil.org/fibo/ontology/FND/Agreements/Contracts/ContractDocument> rdf:type owl:Class ;
                                                                                      rdfs:subClassOf <https://spec.edmcouncil.org/fibo/ontology/FND/Agreements/Contracts/Contract_> ;
                                                                                      rdfs:comment """legal document that records the formal terms and conditions of some contract
"""@en ;
                                                                                      rdfs:label "ContractDocument"@en .


###  https://spec.edmcouncil.org/fibo/ontology/FND/Agreements/Contracts/Contract_
<https://spec.edmcouncil.org/fibo/ontology/FND/Agreements/Contracts/Contract_> rdf:type owl:Class ;
                                                                               rdfs:subClassOf owl:Thing ;
                                                                               rdfs:comment """explanatory note
A contractual relationship is evidenced by (1) an offer, (2) acceptance of the offer, and a (3) valid (legal and valuable) consideration. A contract is a kind of agreement, and as such it embodies the assertion that it has been negotiated, such negotiation having included the presence of some offer and the acceptance of that offer on the part of either or both of the parties.
Contracts are usually written but may be spoken or implied, and generally have to do with employment, sale or lease, or tenancy."""@en ,
                                                                                            "voluntary, deliberate agreement between competent parties to which the parties agree to be legally bound, and for which the parties provide valuable consideration"@en ;
                                                                               rdfs:label "Contract"@en .


###  https://spec.edmcouncil.org/fibo/ontology/FND/Agreements/Contracts/MutualContractualAgreement
<https://spec.edmcouncil.org/fibo/ontology/FND/Agreements/Contracts/MutualContractualAgreement> rdf:type owl:Class ;
                                                                                                rdfs:subClassOf <https://spec.edmcouncil.org/fibo/ontology/FND/Agreements/Contracts/Contract_> ;
                                                                                                owl:disjointWith <https://spec.edmcouncil.org/fibo/ontology/FND/Agreements/Contracts/UnilateralContract> ;
                                                                                                rdfs:comment """synonym(s)
bilateral contract
definition
contract between named parties whose individual rights and obligations are not transferable to another party without prior written permission
explanatory note
A mutual contractual agreement involves an exchange of a promises in which the promises made by each party represent considerations supporting the promises of the other party(ies)."""@en ;
                                                                                                rdfs:label "MutualAgreement"@en .


###  https://spec.edmcouncil.org/fibo/ontology/FND/Agreements/Contracts/TransferableContract
<https://spec.edmcouncil.org/fibo/ontology/FND/Agreements/Contracts/TransferableContract> rdf:type owl:Class ;
                                                                                          rdfs:subClassOf <https://spec.edmcouncil.org/fibo/ontology/FND/Agreements/Contracts/Contract_> ;
                                                                                          rdfs:comment """definition
contract in which the rights and obligations of one party (the holder) may be transferred to another party, which thereby takes on the same rights and obligations with respect to the other party to the contract
explanatory note
Note that the ability to transfer ownership of one side of a contract, and the concept of assignability, are distinct. In one case the contract may be freely traded; in the other case, some legal transfer of rights to a third party takes place, without a change in who are the signatories of a (typically bilateral) contract."""@en ;
                                                                                          rdfs:label "TransferableContract"@en .


###  https://spec.edmcouncil.org/fibo/ontology/FND/Agreements/Contracts/UnilateralContract
<https://spec.edmcouncil.org/fibo/ontology/FND/Agreements/Contracts/UnilateralContract> rdf:type owl:Class ;
                                                                                        rdfs:subClassOf <https://spec.edmcouncil.org/fibo/ontology/FND/Agreements/Contracts/Contract_> ;
                                                                                        rdfs:comment """definition
contract in which one party makes an express promise without securing a reciprocal agreement from the other party(ies)
explanatory note
In a unilateral, or one-sided, contract, one party, known as the offeror, makes a promise in exchange for an act (or abstention from acting) by another party, known as the offeree. If the offeree acts on the offeror's promise, the offeror is legally obligated to fulfill the contract, but an offeree cannot be forced to act (or not act), because no return promise has been made to the offeror. After an offeree has performed, only one enforceable promise exists, that of the offeror."""@en ;
                                                                                        rdfs:label "UnilateralContract"@en .


###  https://spec.edmcouncil.org/fibo/ontology/FND/Agreements/Contracts/VerbalContract
<https://spec.edmcouncil.org/fibo/ontology/FND/Agreements/Contracts/VerbalContract> rdf:type owl:Class ;
                                                                                    rdfs:subClassOf <https://spec.edmcouncil.org/fibo/ontology/FND/Agreements/Contracts/Contract_> ;
                                                                                    owl:disjointWith <https://spec.edmcouncil.org/fibo/ontology/FND/Agreements/Contracts/WrittenContract> ;
                                                                                    rdfs:comment "Contract that exists as a result of some verbal exchange"@en ;
                                                                                    rdfs:label "VerbalContract"@en .


###  https://spec.edmcouncil.org/fibo/ontology/FND/Agreements/Contracts/WrittenContract
<https://spec.edmcouncil.org/fibo/ontology/FND/Agreements/Contracts/WrittenContract> rdf:type owl:Class ;
                                                                                     rdfs:subClassOf <https://spec.edmcouncil.org/fibo/ontology/FND/Agreements/Contracts/Contract_> ;
                                                                                     rdfs:comment "formal contract that is written and signed by the parties thereto"@en ;
                                                                                     rdfs:label "WrittenContract"@en .


###  https://spec.edmcouncil.org/fibo/ontology/FND/Agreements/Contracts/hasEffectiveDate
<https://spec.edmcouncil.org/fibo/ontology/FND/Agreements/Contracts/hasEffectiveDate> rdf:type owl:Class .


###  https://spec.edmcouncil.org/fibo/ontology/FND/Agreements/Contracts/hasExecutionDate
<https://spec.edmcouncil.org/fibo/ontology/FND/Agreements/Contracts/hasExecutionDate> rdf:type owl:Class .


###  https://spec.edmcouncil.org/fibo/ontology/FND/TransactionsExt/REATransactions/EconomicContract
<https://spec.edmcouncil.org/fibo/ontology/FND/TransactionsExt/REATransactions/EconomicContract> rdf:type owl:Class ;
                                                                                                 rdfs:subClassOf <https://spec.edmcouncil.org/fibo/ontology/FND/Agreements/Contracts/MutualContractualAgreement> ;
                                                                                                 rdfs:comment """definition
A contract relating to and governing an economic transaction between two parties. [en]
editorial note
From REA ontology. [en]"""@en ;
                                                                                                 rdfs:label "EconomicContract"@en .


###  https://w3id.org/GConsent#Medium
<https://w3id.org/GConsent#Medium> rdf:type owl:Class ;
                                   rdfs:subClassOf :consent ;
                                   rdfs:comment """Describes the medium through which consent was given/provided. Example: web form, recorded voice, signature on document.
"""@en ;
                                   rdfs:label "Medium "@en .


###  https://w3id.org/GConsent#StatusInvalidForProcessing
<https://w3id.org/GConsent#StatusInvalidForProcessing> rdf:type owl:Class ;
                                                       rdfs:subClassOf :ConsentStatus ;
                                                       rdfs:label "Invalid"@en .


###  https://w3id.org/GConsent#StatusValidForProcessing
<https://w3id.org/GConsent#StatusValidForProcessing> rdf:type owl:Class ;
                                                     rdfs:subClassOf :ConsentStatus ;
                                                     rdfs:label "Valid"@en .


#################################################################
#    Individuals
#################################################################

###  http://ontologies.atb-bremen.de/smashHitCore#ABS_sensor
:ABS_sensor rdf:type owl:NamedIndividual ,
                     <http://mmisw.org/ont/univmemphis/sensor#Motion> ;
            :hasAssociation :k12m0091 .


###  http://ontologies.atb-bremen.de/smashHitCore#Analysing_GPS_for_traffic_detection
:Analysing_GPS_for_traffic_detection rdf:type owl:NamedIndividual ,
                                              <http://www.w3.org/ns/dpv#ServiceProvision> ;
                                     :forDataProcessing :Analysis ,
                                                        :Collection ;
                                     rdfs:comment "Analysing car GPS sensor data for traffic detection"@en .


###  http://ontologies.atb-bremen.de/smashHitCore#Analysis
:Analysis rdf:type owl:NamedIndividual ,
                   rdf:Data_Processing ;
          :hasAssociation :as120098 ,
                          :kg234562 ;
          rdf:hasInputData :GPS .


###  http://ontologies.atb-bremen.de/smashHitCore#Austria
:Austria rdf:type owl:NamedIndividual ,
                  :Country .


###  http://ontologies.atb-bremen.de/smashHitCore#Bavaria
:Bavaria rdf:type owl:NamedIndividual ,
                  :State .


###  http://ontologies.atb-bremen.de/smashHitCore#Brade
:Brade rdf:type owl:NamedIndividual ,
                <http://www.w3.org/ns/prov#Agent> ;
       :hasEmail <http://ontologies.atb-bremen.de/smashHitCore#brade@hotmail.com> ;
       :hasTelephone <http://ontologies.atb-bremen.de/smashHitCore#06759988813065> ;
       :hasStreetAddress :Techniker_Strasse_7 .


###  http://ontologies.atb-bremen.de/smashHitCore#CO2_emission_detection
:CO2_emission_detection rdf:type owl:NamedIndividual ,
                                 <http://www.w3.org/ns/dpv#ServiceProvision> ;
                        :forDataProcessing :Collection .


###  http://ontologies.atb-bremen.de/smashHitCore#CXAM
:CXAM rdf:type owl:NamedIndividual ,
               <http://www.w3.org/ns/prov#Organization> ;
      :hasAssociation :kg234562 ,
                      :kg244562 ,
                      :kg244563 ,
                      :kg244564 ,
                      :kg244565 ;
      :hasRole :Data_Controller .


###  http://ontologies.atb-bremen.de/smashHitCore#Collection
:Collection rdf:type owl:NamedIndividual ,
                     rdf:Data_Processing ;
            :hasAssociation :as120098 ;
            rdf:hasInputData :Fuel_Sensor ,
                             :GPS .


###  http://ontologies.atb-bremen.de/smashHitCore#CompanyABC
:CompanyABC rdf:type owl:NamedIndividual ,
                     <http://www.w3.org/ns/prov#Organization> ;
            :hasEmail <http://ontologies.atb-bremen.de/smashHitCore#companABC@gmail.com> ;
            :hasTelephone <http://ontologies.atb-bremen.de/smashHitCore#06759988813078> ;
            :hasStreetAddress :Hansuntermuhler_Strasse_10 .


###  http://ontologies.atb-bremen.de/smashHitCore#CompanyDEF
:CompanyDEF rdf:type owl:NamedIndividual ,
                     <http://www.w3.org/ns/prov#Organization> ;
            :hasEmail <http://ontologies.atb-bremen.de/smashHitCore#companyDEF@hotmail.com> ;
            :hasTelephone <http://ontologies.atb-bremen.de/smashHitCore#06759988813080> ;
            :hasStreetAddress :Westbhan_Strasse_2 .


###  http://ontologies.atb-bremen.de/smashHitCore#CompanyXYZ
:CompanyXYZ rdf:type owl:NamedIndividual ,
                     <http://www.w3.org/ns/prov#Organization> ;
            :hasAssociation :kg234562 ;
            :hasRole :Data_Requester .


###  http://ontologies.atb-bremen.de/smashHitCore#Data_Controller
:Data_Controller rdf:type owl:NamedIndividual ,
                          :DataController .


###  http://ontologies.atb-bremen.de/smashHitCore#Data_Owner
:Data_Owner rdf:type owl:NamedIndividual ,
                     :DataOwner .


###  http://ontologies.atb-bremen.de/smashHitCore#Data_Provider
:Data_Provider rdf:type owl:NamedIndividual ,
                        :DataProvider .


###  http://ontologies.atb-bremen.de/smashHitCore#Data_Requester
:Data_Requester rdf:type owl:NamedIndividual ,
                         :DataRequester .


###  http://ontologies.atb-bremen.de/smashHitCore#Expired
:Expired rdf:type owl:NamedIndividual ,
                  <https://w3id.org/GConsent#StatusInvalidForProcessing> .


###  http://ontologies.atb-bremen.de/smashHitCore#Fuel
:Fuel rdf:type owl:NamedIndividual ,
               :CarData .


###  http://ontologies.atb-bremen.de/smashHitCore#Fuel_Sensor
:Fuel_Sensor rdf:type owl:NamedIndividual ,
                      :CarData .


###  http://ontologies.atb-bremen.de/smashHitCore#Fuel_consumption_in_traffic
:Fuel_consumption_in_traffic rdf:type owl:NamedIndividual ,
                                      <http://www.w3.org/ns/dpv#ServiceProvision> ;
                             :forDataProcessing :Analysis ,
                                                :Collection .


###  http://ontologies.atb-bremen.de/smashHitCore#Fuel_usage_collection
:Fuel_usage_collection rdf:type owl:NamedIndividual ,
                                <http://www.w3.org/ns/dpv#Collect> ;
                       rdf:hasInputData :Fuel .


###  http://ontologies.atb-bremen.de/smashHitCore#GPS
:GPS rdf:type owl:NamedIndividual ,
              :CarData .


###  http://ontologies.atb-bremen.de/smashHitCore#GPS_and_Fuel
:GPS_and_Fuel rdf:type owl:NamedIndividual ,
                       <http://www.w3.org/ns/dpv#Combine> ;
              rdf:hasInputData :Fuel_Sensor ,
                               :GPS .


###  http://ontologies.atb-bremen.de/smashHitCore#George
:George rdf:type owl:NamedIndividual ,
                 <http://www.w3.org/ns/prov#Agent> ;
        :hasEmail <http://ontologies.atb-bremen.de/smashHitCore#george@hotmail.com> ;
        :hasTelephone <http://ontologies.atb-bremen.de/smashHitCore#06759988813085> ;
        :hasStreetAddress :Leopold_Strasse_15 .


###  http://ontologies.atb-bremen.de/smashHitCore#Germany
:Germany rdf:type owl:NamedIndividual ,
                  :Country .


###  http://ontologies.atb-bremen.de/smashHitCore#Government_Website
:Government_Website rdf:type owl:NamedIndividual ,
                             <http://purl.org/adaptcentre/openscience/ontologies/consent#AppBased> .


###  http://ontologies.atb-bremen.de/smashHitCore#ID_234562
:ID_234562 rdf:type owl:NamedIndividual ;
           <http://purl.org/dc/terms/identifier> :kg234562 .


###  http://ontologies.atb-bremen.de/smashHitCore#ID_244562
:ID_244562 rdf:type owl:NamedIndividual ;
           <http://purl.org/dc/terms/identifier> :kg244562 .


###  http://ontologies.atb-bremen.de/smashHitCore#ID_244563
:ID_244563 rdf:type owl:NamedIndividual ;
           <http://purl.org/dc/terms/identifier> :kg244563 ,
                                                 :kg244564 ,
                                                 :kg244565 .


###  http://ontologies.atb-bremen.de/smashHitCore#ID_244564
:ID_244564 rdf:type owl:NamedIndividual .


###  http://ontologies.atb-bremen.de/smashHitCore#ID_244565
:ID_244565 rdf:type owl:NamedIndividual .


###  http://ontologies.atb-bremen.de/smashHitCore#InValid
:InValid rdf:type owl:NamedIndividual ,
                  :hasContractStatus .


###  http://ontologies.atb-bremen.de/smashHitCore#Innsbruck
:Innsbruck rdf:type owl:NamedIndividual ,
                    :City .


###  http://ontologies.atb-bremen.de/smashHitCore#Invalidated
:Invalidated rdf:type owl:NamedIndividual ,
                      <https://w3id.org/GConsent#StatusInvalidForProcessing> .


###  http://ontologies.atb-bremen.de/smashHitCore#JDLimited
:JDLimited rdf:type owl:NamedIndividual ,
                    <http://www.w3.org/ns/prov#Organization> ;
           :hasRole :Data_Controller .


###  http://ontologies.atb-bremen.de/smashHitCore#JJDoe
:JJDoe rdf:type owl:NamedIndividual ,
                <http://www.w3.org/ns/dpv#Username> .


###  http://ontologies.atb-bremen.de/smashHitCore#JJKLimited
:JJKLimited rdf:type owl:NamedIndividual ,
                     <http://www.w3.org/ns/prov#Organization> ;
            :hasRole :Data_Requester .


###  http://ontologies.atb-bremen.de/smashHitCore#JackDoe
:JackDoe rdf:type owl:NamedIndividual ,
                  <http://www.w3.org/ns/prov#Person> ;
         :hasEmail <http://ontologies.atb-bremen.de/smashHitCore#jackDoe123@gmail.com> ;
         :hasRole :Data_Provider ;
         :hasTelephone <http://ontologies.atb-bremen.de/smashHitCore#095944598> ;
         :hasUsername :JJDoe .


###  http://ontologies.atb-bremen.de/smashHitCore#Jack_Jones
:Jack_Jones rdf:type owl:NamedIndividual ,
                     <http://www.w3.org/ns/prov#Person> .


###  http://ontologies.atb-bremen.de/smashHitCore#JaneDoe
:JaneDoe rdf:type owl:NamedIndividual ,
                  <http://www.w3.org/ns/prov#Person> ;
         :hasEmail <http://ontologies.atb-bremen.de/smashHitCore#janedoe@gmail.com> ;
         :hasTelephone <http://ontologies.atb-bremen.de/smashHitCore#5550002929> ;
         :hasUsername :JaneDoe1 .


###  http://ontologies.atb-bremen.de/smashHitCore#JaneDoe1
:JaneDoe1 rdf:type owl:NamedIndividual ,
                   <http://www.w3.org/ns/dpv#Username> .


###  http://ontologies.atb-bremen.de/smashHitCore#JanneDoe
:JanneDoe rdf:type owl:NamedIndividual ,
                   <http://www.w3.org/ns/prov#Person> ;
          :hasEmail <http://ontologies.atb-bremen.de/smashHitCore#jannedoe2@gmail.com> ;
          :hasPersonalData :xxy23909 ,
                           <http://ontologies.atb-bremen.de/smashHitCore#115986kls> ;
          :hasRole :Data_Provider ;
          :hasTelephone <http://ontologies.atb-bremen.de/smashHitCore#993939904> ;
          :hasUsername :janneDoe2 .


###  http://ontologies.atb-bremen.de/smashHitCore#JohnDoe123
:JohnDoe123 rdf:type owl:NamedIndividual ,
                     <http://www.w3.org/ns/dpv#Username> .


###  http://ontologies.atb-bremen.de/smashHitCore#John_Doe
:John_Doe rdf:type owl:NamedIndividual ,
                   <http://www.w3.org/ns/prov#Person> ;
          :hasEmail <http://ontologies.atb-bremen.de/smashHitCore#johnDoe123@gmail.com> ;
          :hasRole :Data_Provider ;
          :hasTelephone <http://ontologies.atb-bremen.de/smashHitCore#009938484> ;
          :hasUsername :JohnDoe123 .


###  http://ontologies.atb-bremen.de/smashHitCore#Madrid
:Madrid rdf:type owl:NamedIndividual ,
                 :City .


###  http://ontologies.atb-bremen.de/smashHitCore#MobileApp123
:MobileApp123 rdf:type owl:NamedIndividual ,
                       <http://purl.org/adaptcentre/openscience/ontologies/consent#AppBased> .


###  http://ontologies.atb-bremen.de/smashHitCore#Munich
:Munich rdf:type owl:NamedIndividual ,
                 :City .


###  http://ontologies.atb-bremen.de/smashHitCore#Munich_City_Concil
:Munich_City_Concil rdf:type owl:NamedIndividual ,
                             <http://www.w3.org/ns/prov#Organization> .


###  http://ontologies.atb-bremen.de/smashHitCore#MyConsentApp1
:MyConsentApp1 rdf:type owl:NamedIndividual ,
                        <http://purl.org/adaptcentre/openscience/ontologies/consent#AppBased> .


###  http://ontologies.atb-bremen.de/smashHitCore#NotGiven
:NotGiven rdf:type owl:NamedIndividual ,
                   <https://w3id.org/GConsent#StatusInvalidForProcessing> .


###  http://ontologies.atb-bremen.de/smashHitCore#Paper_Form
:Paper_Form rdf:type owl:NamedIndividual ,
                     <http://purl.org/adaptcentre/openscience/ontologies/consent#Paper> .


###  http://ontologies.atb-bremen.de/smashHitCore#Refused
:Refused rdf:type owl:NamedIndividual ,
                  <https://w3id.org/GConsent#StatusInvalidForProcessing> .


###  http://ontologies.atb-bremen.de/smashHitCore#Requested
:Requested rdf:type owl:NamedIndividual ,
                    <https://w3id.org/GConsent#StatusInvalidForProcessing> .


###  http://ontologies.atb-bremen.de/smashHitCore#Road_Condition_Analysis
:Road_Condition_Analysis rdf:type owl:NamedIndividual ,
                                  <http://www.w3.org/ns/dpv#ServiceProvision> ;
                         :forDataProcessing :Analysis .


###  http://ontologies.atb-bremen.de/smashHitCore#Spain
:Spain rdf:type owl:NamedIndividual ,
                :Country .


###  http://ontologies.atb-bremen.de/smashHitCore#Tyrol
:Tyrol rdf:type owl:NamedIndividual ,
                :State .


###  http://ontologies.atb-bremen.de/smashHitCore#Valid
:Valid rdf:type owl:NamedIndividual ,
                :hasContractStatus .


###  http://ontologies.atb-bremen.de/smashHitCore#WebAppExample
:WebAppExample rdf:type owl:NamedIndividual ,
                        <http://purl.org/adaptcentre/openscience/ontologies/consent#AppBased> .


###  http://ontologies.atb-bremen.de/smashHitCore#Withdrawn
:Withdrawn rdf:type owl:NamedIndividual ,
                    <https://w3id.org/GConsent#StatusInvalidForProcessing> .


###  http://ontologies.atb-bremen.de/smashHitCore#WrittenContract
:WrittenContract rdf:type owl:NamedIndividual ,
                          <https://spec.edmcouncil.org/fibo/ontology/FND/Agreements/Contracts/WrittenContract> .


###  http://ontologies.atb-bremen.de/smashHitCore#as120098
:as120098 rdf:type owl:NamedIndividual ,
                   :ConsentID ;
          :atCity :Innsbruck ;
          :atCountry :Austria ;
          :atState :Tyrol ;
          :hasDataController :CompanyXYZ ,
                             :JDLimited ;
          :hasExpiry <http://ontologies.atb-bremen.de/smashHitCore#2months> ;
          :inMedium :MyConsentApp1 ;
          :isAboutData :Fuel ,
                       :GPS ;
          :isProvidedBy :JackDoe ;
          :requestedBy :JJKLimited ;
          <http://www.w3.org/ns/dpv#hasPurpose> :Analysing_GPS_for_traffic_detection .


###  http://ontologies.atb-bremen.de/smashHitCore#dalicc
:dalicc rdf:type owl:NamedIndividual ,
                 :license .


###  http://ontologies.atb-bremen.de/smashHitCore#f0200gh
:f0200gh rdf:type owl:NamedIndividual ,
                  :ConsentID ;
         :atCity :Madrid ;
         :atCountry :Spain ;
         :hasDataController :CXAM ;
         :hasExpiry <http://ontologies.atb-bremen.de/smashHitCore#1week> ;
         :isAboutData :Fuel ;
         :isProvidedBy :Jack_Jones ;
         :requestedBy :CXAM ;
         <http://www.w3.org/ns/dpv#hasPurpose> :CO2_emission_detection .


###  http://ontologies.atb-bremen.de/smashHitCore#f115986kls3
:f115986kls3 rdf:type owl:NamedIndividual ,
                      <http://www.w3.org/ns/dpv#OfficialID> .


###  http://ontologies.atb-bremen.de/smashHitCore#hasAmendment
:hasAmendment rdf:type owl:NamedIndividual .


###  http://ontologies.atb-bremen.de/smashHitCore#hasConfidentialityObligation
:hasConfidentialityObligation rdf:type owl:NamedIndividual .


###  http://ontologies.atb-bremen.de/smashHitCore#hasDataProtection
:hasDataProtection rdf:type owl:NamedIndividual .


###  http://ontologies.atb-bremen.de/smashHitCore#hasLimitationOnUse
:hasLimitationOnUse rdf:type owl:NamedIndividual .


###  http://ontologies.atb-bremen.de/smashHitCore#hasMethodOfNotice
:hasMethodOfNotice rdf:type owl:NamedIndividual .


###  http://ontologies.atb-bremen.de/smashHitCore#hasNoThirdPartyBeneficiaries
:hasNoThirdPartyBeneficiaries rdf:type owl:NamedIndividual .


###  http://ontologies.atb-bremen.de/smashHitCore#hasPermittedDisclosure
:hasPermittedDisclosure rdf:type owl:NamedIndividual .


###  http://ontologies.atb-bremen.de/smashHitCore#hasReceiptOfNotice
:hasReceiptOfNotice rdf:type owl:NamedIndividual .


###  http://ontologies.atb-bremen.de/smashHitCore#hasSeverability
:hasSeverability rdf:type owl:NamedIndividual .


###  http://ontologies.atb-bremen.de/smashHitCore#hasTerminationForInsolvency
:hasTerminationForInsolvency rdf:type owl:NamedIndividual .


###  http://ontologies.atb-bremen.de/smashHitCore#hasTerminationForMaterialBreach
:hasTerminationForMaterialBreach rdf:type owl:NamedIndividual .


###  http://ontologies.atb-bremen.de/smashHitCore#hasTerminationOnNotice
:hasTerminationOnNotice rdf:type owl:NamedIndividual .


###  http://ontologies.atb-bremen.de/smashHitCore#hasWaiver
:hasWaiver rdf:type owl:NamedIndividual .


###  http://ontologies.atb-bremen.de/smashHitCore#janneDoe2
:janneDoe2 rdf:type owl:NamedIndividual ,
                    <http://www.w3.org/ns/dpv#Username> .


###  http://ontologies.atb-bremen.de/smashHitCore#k12m0091
:k12m0091 rdf:type owl:NamedIndividual ,
                   :ConsentID ;
          :atCity :Munich ;
          :atCountry :Germany ;
          :atState :Bavaria ;
          :hasDataController :JDLimited ;
          :hasExpiry <http://ontologies.atb-bremen.de/smashHitCore#5months> ;
          :inMedium :Government_Website ;
          :isAboutData :GPS ;
          :isProvidedBy :JaneDoe ;
          <http://www.w3.org/ns/dpv#hasPurpose> :Fuel_consumption_in_traffic .


###  http://ontologies.atb-bremen.de/smashHitCore#kg234562
:kg234562 rdf:type owl:NamedIndividual ,
                   :ConsentID ;
          :atCity :Innsbruck ;
          :atCountry :Austria ;
          :hasDataController :CXAM ;
          :hasExpiry <http://ontologies.atb-bremen.de/smashHitCore#10days> ;
          :inMedium :MobileApp123 ;
          :isAboutData :GPS ;
          :isProvidedBy :JaneDoe ;
          :requestedBy :CompanyXYZ ;
          <http://purl.org/dc/terms/identifier> :ID_234562 ;
          <http://www.w3.org/ns/dpv#hasPurpose> :Analysing_GPS_for_traffic_detection .


###  http://ontologies.atb-bremen.de/smashHitCore#kg244562
:kg244562 rdf:type owl:NamedIndividual ,
                   :ContractId ;
          :hasAmendment :hasAmendment ;
          :hasConfidentialityObligation :hasConfidentialityObligation ;
          :hasContractStatus :Valid ;
          :hasDataController :CXAM ;
          :hasDataProtection :hasDataProtection ;
          :hasLimitationOnUse :hasLimitationOnUse ;
          :hasMethodOfNotice :hasMethodOfNotice ;
          :hasMinimumDuration <http://ontologies.atb-bremen.de/smashHitCore#1_year> ;
          :hasNoThirdPartyBeneficiaries :hasNoThirdPartyBeneficiaries ;
          :hasPermittedDisclosure :hasPermittedDisclosure ;
          :hasReceiptOfNotice :hasReceiptOfNotice ;
          :hasSeverability :hasSeverability ;
          :hasTerminationForInsolvency :hasTerminationForInsolvency ;
          :hasTerminationForMaterialBreach :hasTerminationForMaterialBreach ;
          :hasTerminationOnNotice :hasTerminationOnNotice ;
          :hasWaiver :hasWaiver ;
          :inMedium :MobileApp123 ;
          <http://purl.org/dc/terms/identifier> :ID_244562 ;
          <http://www.w3.org/ns/dcat#endDate> <http://ontologies.atb-bremen.de/smashHitCore#05-05-2022> ;
          <http://www.w3.org/ns/dcat#startDate> <http://ontologies.atb-bremen.de/smashHitCore#05-05-2021> ;
          <https://spec.edmcouncil.org/fibo/ontology/FND/Agreements/Contracts/hasEffectiveDate> <http://ontologies.atb-bremen.de/smashHitCore#05-05-2021> ;
          <https://spec.edmcouncil.org/fibo/ontology/FND/Agreements/Contracts/hasExecutionDate> <http://ontologies.atb-bremen.de/smashHitCore#05-05-2021> ;
          :ContractProvider :Brade ;
          :ContractRequester :CompanyABC ;
          :contractType :WrittenContract ;
          :forPurpose "Creation of Contract for Vehicle data" .


###  http://ontologies.atb-bremen.de/smashHitCore#kg244563
:kg244563 rdf:type owl:NamedIndividual ,
                   :ContractId ;
          :hasAmendment :hasAmendment ;
          :hasConfidentialityObligation :hasConfidentialityObligation ;
          :hasContractStatus :Valid ;
          :hasDataController :CXAM ;
          :hasDataProtection :hasDataProtection ;
          :hasLimitationOnUse :hasLimitationOnUse ;
          :hasMethodOfNotice :hasMethodOfNotice ;
          :hasMinimumDuration <http://ontologies.atb-bremen.de/smashHitCore#1_year> ;
          :hasNoThirdPartyBeneficiaries :hasNoThirdPartyBeneficiaries ;
          :hasPermittedDisclosure :hasPermittedDisclosure ;
          :hasReceiptOfNotice :hasReceiptOfNotice ;
          :hasSeverability :hasSeverability ;
          :hasTerminationForInsolvency :hasTerminationForInsolvency ;
          :hasTerminationForMaterialBreach :hasTerminationForMaterialBreach ;
          :hasTerminationOnNotice :hasTerminationOnNotice ;
          :hasWaiver :hasWaiver ;
          :inMedium :MobileApp123 ;
          <http://purl.org/dc/terms/identifier> :ID_244563 ;
          <http://www.w3.org/ns/dcat#endDate> <http://ontologies.atb-bremen.de/smashHitCore#05-05-2022> ;
          <http://www.w3.org/ns/dcat#startDate> <http://ontologies.atb-bremen.de/smashHitCore#05-05-2021> ;
          <https://spec.edmcouncil.org/fibo/ontology/FND/Agreements/Contracts/hasEffectiveDate> <http://ontologies.atb-bremen.de/smashHitCore#05-05-2021> ;
          <https://spec.edmcouncil.org/fibo/ontology/FND/Agreements/Contracts/hasExecutionDate> <http://ontologies.atb-bremen.de/smashHitCore#05-05-2021> ;
          :ContractProvider :Brade ;
          :ContractRequester :CompanyABC ,
                             :CompanyDEF ;
          :contractType :WrittenContract ;
          :forPurpose "Creation of Contract for Vehicle data" .


###  http://ontologies.atb-bremen.de/smashHitCore#kg244564
:kg244564 rdf:type owl:NamedIndividual ,
                   :ContractId ;
          :hasAmendment :hasAmendment ;
          :hasConfidentialityObligation :hasConfidentialityObligation ;
          :hasContractStatus :Valid ;
          :hasDataController :CXAM ;
          :hasDataProtection :hasDataProtection ;
          :hasLimitationOnUse :hasLimitationOnUse ;
          :hasMethodOfNotice :hasMethodOfNotice ;
          :hasMinimumDuration <http://ontologies.atb-bremen.de/smashHitCore#1_year> ;
          :hasNoThirdPartyBeneficiaries :hasNoThirdPartyBeneficiaries ;
          :hasPermittedDisclosure :hasPermittedDisclosure ;
          :hasReceiptOfNotice :hasReceiptOfNotice ;
          :hasSeverability :hasSeverability ;
          :hasTerminationForInsolvency :hasTerminationForInsolvency ;
          :hasTerminationForMaterialBreach :hasTerminationForMaterialBreach ;
          :hasTerminationOnNotice :hasTerminationOnNotice ;
          :hasWaiver :hasWaiver ;
          :inMedium :MobileApp123 ;
          <http://purl.org/dc/terms/identifier> :ID_244564 ;
          <http://www.w3.org/ns/dcat#endDate> <http://ontologies.atb-bremen.de/smashHitCore#05-05-2022> ;
          <http://www.w3.org/ns/dcat#startDate> <http://ontologies.atb-bremen.de/smashHitCore#05-05-2021> ;
          <https://spec.edmcouncil.org/fibo/ontology/FND/Agreements/Contracts/hasEffectiveDate> <http://ontologies.atb-bremen.de/smashHitCore#05-05-2021> ;
          <https://spec.edmcouncil.org/fibo/ontology/FND/Agreements/Contracts/hasExecutionDate> <http://ontologies.atb-bremen.de/smashHitCore#05-05-2021> ;
          :ContractProvider :Brade ,
                            :George ;
          :ContractRequester :CompanyABC ;
          :contractType :WrittenContract ;
          :forPurpose "Creation of Contract for Vehicle data" .


###  http://ontologies.atb-bremen.de/smashHitCore#kg244565
:kg244565 rdf:type owl:NamedIndividual ,
                   :ContractId ;
          :hasAmendment :hasAmendment ;
          :hasConfidentialityObligation :hasConfidentialityObligation ;
          :hasContractStatus :Valid ;
          :hasDataController :CXAM ;
          :hasDataProtection :hasDataProtection ;
          :hasLimitationOnUse :hasLimitationOnUse ;
          :hasMethodOfNotice :hasMethodOfNotice ;
          :hasMinimumDuration <http://ontologies.atb-bremen.de/smashHitCore#1_year> ;
          :hasNoThirdPartyBeneficiaries :hasNoThirdPartyBeneficiaries ;
          :hasPermittedDisclosure :hasPermittedDisclosure ;
          :hasReceiptOfNotice :hasReceiptOfNotice ;
          :hasSeverability :hasSeverability ;
          :hasTerminationForInsolvency :hasTerminationForInsolvency ;
          :hasTerminationForMaterialBreach :hasTerminationForMaterialBreach ;
          :hasTerminationOnNotice :hasTerminationOnNotice ;
          :hasWaiver :hasWaiver ;
          :inMedium :MobileApp123 ;
          <http://purl.org/dc/terms/identifier> :ID_244565 ;
          <http://www.w3.org/ns/dcat#endDate> <http://ontologies.atb-bremen.de/smashHitCore#05-05-2022> ;
          <http://www.w3.org/ns/dcat#startDate> <http://ontologies.atb-bremen.de/smashHitCore#05-05-2021> ;
          <https://spec.edmcouncil.org/fibo/ontology/FND/Agreements/Contracts/hasEffectiveDate> <http://ontologies.atb-bremen.de/smashHitCore#05-05-2021> ;
          <https://spec.edmcouncil.org/fibo/ontology/FND/Agreements/Contracts/hasExecutionDate> <http://ontologies.atb-bremen.de/smashHitCore#05-05-2021> ;
          :ContractProvider :Brade ,
                            :George ;
          :ContractRequester :CompanyABC ,
                             :CompanyDEF ;
          :contractType :WrittenContract ;
          :forPurpose "Creation of Contract for Vehicle data" .


###  http://ontologies.atb-bremen.de/smashHitCore#kkkjskskmw
:kkkjskskmw rdf:type owl:NamedIndividual ,
                     :Hash .


###  http://ontologies.atb-bremen.de/smashHitCore#kls123976
:kls123976 rdf:type owl:NamedIndividual ,
                    <http://www.w3.org/ns/dpv#OfficialID> .


###  http://ontologies.atb-bremen.de/smashHitCore#latitude
:latitude rdf:type owl:NamedIndividual ,
                   <http://mmisw.org/ont/univmemphis/sensor#GPS> ;
          :hasAssociation :k12m0091 .


###  http://ontologies.atb-bremen.de/smashHitCore#license
:license rdf:type owl:NamedIndividual ,
                  :dalicc .


###  http://ontologies.atb-bremen.de/smashHitCore#longitude
:longitude rdf:type owl:NamedIndividual ,
                    <http://mmisw.org/ont/univmemphis/sensor#GPS> ;
           :hasAssociation :k12m0091 .


###  http://ontologies.atb-bremen.de/smashHitCore#temperature_sensor
:temperature_sensor rdf:type owl:NamedIndividual ,
                             :BuildingData .


###  http://ontologies.atb-bremen.de/smashHitCore#xxy23009
:xxy23009 rdf:type owl:NamedIndividual ,
                   <http://www.w3.org/ns/dpv#UID> .


###  http://ontologies.atb-bremen.de/smashHitCore#xxy23909
:xxy23909 rdf:type owl:NamedIndividual ,
                   <http://www.w3.org/ns/dpv#UID> .


###  http://ontologies.atb-bremen.de/smashHitCore#xyz23809
:xyz23809 rdf:type owl:NamedIndividual ,
                   <http://www.w3.org/ns/dpv#UID> .


###  http://ontologies.atb-bremen.de/smashHitCore#009938484
<http://ontologies.atb-bremen.de/smashHitCore#009938484> rdf:type owl:NamedIndividual ,
                                                                  :TelephoneNumber .


###  http://ontologies.atb-bremen.de/smashHitCore#02/04/2021
<http://ontologies.atb-bremen.de/smashHitCore#02/04/2021> rdf:type owl:NamedIndividual ,
                                                                   <http://purl.org/adaptcentre/openscience/ontologies/consent#Time> .


###  http://ontologies.atb-bremen.de/smashHitCore#05-05-2021
<http://ontologies.atb-bremen.de/smashHitCore#05-05-2021> rdf:type owl:NamedIndividual .


###  http://ontologies.atb-bremen.de/smashHitCore#05-05-2022
<http://ontologies.atb-bremen.de/smashHitCore#05-05-2022> rdf:type owl:NamedIndividual .


###  http://ontologies.atb-bremen.de/smashHitCore#05/05/2021
<http://ontologies.atb-bremen.de/smashHitCore#05/05/2021> rdf:type owl:NamedIndividual ,
                                                                   <http://www.w3.org/ns/dcat#startDate> ,
                                                                   <https://spec.edmcouncil.org/fibo/ontology/FND/Agreements/Contracts/hasEffectiveDate> ,
                                                                   <https://spec.edmcouncil.org/fibo/ontology/FND/Agreements/Contracts/hasExecutionDate> .


###  http://ontologies.atb-bremen.de/smashHitCore#05/05/2024
<http://ontologies.atb-bremen.de/smashHitCore#05/05/2024> rdf:type owl:NamedIndividual ,
                                                                   <http://www.w3.org/ns/dcat#endDate> .


###  http://ontologies.atb-bremen.de/smashHitCore#06759988813065
<http://ontologies.atb-bremen.de/smashHitCore#06759988813065> rdf:type owl:NamedIndividual ,
                                                                       :hasTelephone .


###  http://ontologies.atb-bremen.de/smashHitCore#06759988813078
<http://ontologies.atb-bremen.de/smashHitCore#06759988813078> rdf:type owl:NamedIndividual ,
                                                                       :hasTelephone .


###  http://ontologies.atb-bremen.de/smashHitCore#06759988813080
<http://ontologies.atb-bremen.de/smashHitCore#06759988813080> rdf:type owl:NamedIndividual ,
                                                                       :hasTelephone .


###  http://ontologies.atb-bremen.de/smashHitCore#06759988813085
<http://ontologies.atb-bremen.de/smashHitCore#06759988813085> rdf:type owl:NamedIndividual ,
                                                                       :hasTelephone .


###  http://ontologies.atb-bremen.de/smashHitCore#095944598
<http://ontologies.atb-bremen.de/smashHitCore#095944598> rdf:type owl:NamedIndividual ,
                                                                  :TelephoneNumber .


###  http://ontologies.atb-bremen.de/smashHitCore#1_Year
<http://ontologies.atb-bremen.de/smashHitCore#1_Year> rdf:type owl:NamedIndividual ;
                                                      :hasAssociation :kg244562 .


###  http://ontologies.atb-bremen.de/smashHitCore#1_year
<http://ontologies.atb-bremen.de/smashHitCore#1_year> rdf:type owl:NamedIndividual ,
                                                               :hasMinimumDuration ;
                                                      :hasAssociation :kg244565 .


###  http://ontologies.atb-bremen.de/smashHitCore#1week
<http://ontologies.atb-bremen.de/smashHitCore#1week> rdf:type owl:NamedIndividual ,
                                                              <http://purl.org/dc/terms/PeriodOfTime> .


###  http://ontologies.atb-bremen.de/smashHitCore#10days
<http://ontologies.atb-bremen.de/smashHitCore#10days> rdf:type owl:NamedIndividual ,
                                                               <http://purl.org/dc/terms/PeriodOfTime> ;
                                                      :hasAssociation :kg234562 .


###  http://ontologies.atb-bremen.de/smashHitCore#10/05/2021
<http://ontologies.atb-bremen.de/smashHitCore#10/05/2021> rdf:type owl:NamedIndividual ,
                                                                   <http://purl.org/adaptcentre/openscience/ontologies/consent#Time> .


###  http://ontologies.atb-bremen.de/smashHitCore#115986kls
<http://ontologies.atb-bremen.de/smashHitCore#115986kls> rdf:type owl:NamedIndividual ,
                                                                  <http://www.w3.org/ns/dpv#OfficialID> .


###  http://ontologies.atb-bremen.de/smashHitCore#2months
<http://ontologies.atb-bremen.de/smashHitCore#2months> rdf:type owl:NamedIndividual ,
                                                                <http://purl.org/dc/terms/PeriodOfTime> .


###  http://ontologies.atb-bremen.de/smashHitCore#22/03/2021
<http://ontologies.atb-bremen.de/smashHitCore#22/03/2021> rdf:type owl:NamedIndividual ,
                                                                   <http://purl.org/adaptcentre/openscience/ontologies/consent#Time> .


###  http://ontologies.atb-bremen.de/smashHitCore#5days
<http://ontologies.atb-bremen.de/smashHitCore#5days> rdf:type owl:NamedIndividual ,
                                                              <http://purl.org/dc/terms/PeriodOfTime> .


###  http://ontologies.atb-bremen.de/smashHitCore#5months
<http://ontologies.atb-bremen.de/smashHitCore#5months> rdf:type owl:NamedIndividual ,
                                                                <http://purl.org/dc/terms/PeriodOfTime> .


###  http://ontologies.atb-bremen.de/smashHitCore#5550002929
<http://ontologies.atb-bremen.de/smashHitCore#5550002929> rdf:type owl:NamedIndividual ,
                                                                   :TelephoneNumber .


###  http://ontologies.atb-bremen.de/smashHitCore#6_month
<http://ontologies.atb-bremen.de/smashHitCore#6_month> rdf:type owl:NamedIndividual ,
                                                                :hasMinimumDuration ;
                                                       :hasAssociation :kg244563 ,
                                                                       :kg244564 .


###  http://ontologies.atb-bremen.de/smashHitCore#993939904
<http://ontologies.atb-bremen.de/smashHitCore#993939904> rdf:type owl:NamedIndividual ,
                                                                  :TelephoneNumber .


###  http://ontologies.atb-bremen.de/smashHitCore#brade@hotmail.com
<http://ontologies.atb-bremen.de/smashHitCore#brade@hotmail.com> rdf:type owl:NamedIndividual ,
                                                                          :hasEmail .


###  http://ontologies.atb-bremen.de/smashHitCore#companABC@gmail.com
<http://ontologies.atb-bremen.de/smashHitCore#companABC@gmail.com> rdf:type owl:NamedIndividual .


###  http://ontologies.atb-bremen.de/smashHitCore#companyABC@gmail.com
<http://ontologies.atb-bremen.de/smashHitCore#companyABC@gmail.com> rdf:type owl:NamedIndividual ,
                                                                             :hasEmail .


###  http://ontologies.atb-bremen.de/smashHitCore#companyDEF@hotmail.com
<http://ontologies.atb-bremen.de/smashHitCore#companyDEF@hotmail.com> rdf:type owl:NamedIndividual ,
                                                                               :hasEmail .


###  http://ontologies.atb-bremen.de/smashHitCore#george@hotmail.com
<http://ontologies.atb-bremen.de/smashHitCore#george@hotmail.com> rdf:type owl:NamedIndividual ,
                                                                           :hasEmail .


###  http://ontologies.atb-bremen.de/smashHitCore#jackDoe123@gmail.com
<http://ontologies.atb-bremen.de/smashHitCore#jackDoe123@gmail.com> rdf:type owl:NamedIndividual ,
                                                                             <http://www.w3.org/ns/dpv#EmailAddress> .


###  http://ontologies.atb-bremen.de/smashHitCore#janedoe@gmail.com
<http://ontologies.atb-bremen.de/smashHitCore#janedoe@gmail.com> rdf:type owl:NamedIndividual ,
                                                                          <http://www.w3.org/ns/dpv#EmailAddress> .


###  http://ontologies.atb-bremen.de/smashHitCore#jannedoe2@gmail.com
<http://ontologies.atb-bremen.de/smashHitCore#jannedoe2@gmail.com> rdf:type owl:NamedIndividual ,
                                                                            <http://www.w3.org/ns/dpv#EmailAddress> .


###  http://ontologies.atb-bremen.de/smashHitCore#johnDoe123@gmail.com
<http://ontologies.atb-bremen.de/smashHitCore#johnDoe123@gmail.com> rdf:type owl:NamedIndividual ,
                                                                             <http://www.w3.org/ns/dpv#EmailAddress> .


#################################################################
#    Annotations
#################################################################

<dct:Location> rdfs:comment "A spatial region or named place."@en .


<dct:PeriodOfTime> rdfs:comment "An interval of time that is named or defined by its start and end dates."@en .


<dct:accessRights> rdfs:comment "A rights statement that concerns how the distribution is accessed."@en .


<dct:modified> rdfs:comment "Most recent date on which the distribution was changed, updated or modified."@en .


<dct:rights> rdfs:comment "Information about rights held in and over the distribution."@en .


:forPurpose rdfs:label "PurposeLimitation"@en .


:given rdfs:label "Given"@en .


:hasAmendment rdfs:comment "This agreement can be amended only by a writing signed by both parties."@en ;
              rdfs:label "hasAmendment"@en .


:hasConfidentialityObligation rdfs:comment "The receiving party will hold the Confidential Information in confidence."@en ;
                              rdfs:label "hasConfidentialityObligation"@en .


:hasContractStatus rdfs:comment "Specify the status of a contract"@en ;
                   rdfs:label "hasContractStatus"@en .


:hasDataProtection rdfs:comment " First Party will implement appropriate safeguards to prevent unauthorized access to, use of, or disclosure of the Protected Information. "@en ;
                   rdfs:label "hasDataProtection"@en .


:hasLimitationOnUse rdfs:comment "The receiving party will use the Confidential Information only in accordance with the terms of this agreement and solely for the Purpose."@en .


:hasMethodOfNotice rdfs:comment "The parties will give all notices and communications between the parties in writing by (i) personal delivery, (ii) a nationally-recognized, next-day courier service, (iii) first-class registered or certified mail, postage prepaid to the address that a party has notified to be that party's address for the purposes of this section."@en ;
                   rdfs:label "hasMethodOfNotice"@en .


:hasMinimumDuration rdfs:comment "Specify minimum duration of a contract"@en ;
                    rdfs:label "hasMinimumDuration"@en .


:hasNoThirdPartyBeneficiaries rdfs:comment "Unless explicitly stated otherwise elsewhere in this agreement, no Person other than the parties themselves has any rights or remedies under this agreement."@en ;
                              rdfs:label "hasNoThirdPartyBeneficiaries"@en .


:hasPermittedDisclosure rdfs:comment "The receiving party may disclose Confidential Information if and to the extent that the disclosing party consents in writing to such disclosure, or to the receiving party's officers, directors, employees, Affiliates, or representatives who have a need to know the Confidential Information, have been informed of the confidentiality obligations of this agreement,  and  agree to be bound by the term of this agreement."@en ;
                        rdfs:label "hasPermittedDisclosure"@en .


:hasReceiptOfNotice rdfs:comment "A notice given under this agreement will be effective on the (i) other party's receipt of it, or (ii) if mailed, the earlier of the other party's receipt of it and the fifth business day after mailing it. "@en ;
                    rdfs:label "hasReceiptOfNotice"@en .


:hasSeverability rdfs:comment "If any part of this agreement is declared unenforceable or invalid, the remainder will continue to be valid and enforceable."@en ;
                 rdfs:label "hasSeverability"@en .


:hasTerminationForInsolvency rdfs:comment "If either party becomes insolvent, bankrupt, or enters receivership, dissolution, or liquidation, the other party may terminate this agreement with immediate effect."@en ;
                             rdfs:label "hasTerminationForInsolvency"@en .


:hasTerminationForMaterialBreach rdfs:comment "Each party may terminate this agreement with immediate effect by delivering notice of the termination to the other party, if the other party fails to perform, has made or makes any inaccuracy in, or otherwise materially breaches, any of its obligations, covenants, or representations, and the failure, inaccuracy, or breach continues for a period of  [[BREACH CONTINUATION DAYS] Business Days' after the injured party delivers notice to the breaching party reasonably detailing the breach."@en ;
                                 rdfs:label "hasTerminationForMaterialBreach"@en .


:hasTerminationOnNotice rdfs:comment "Either party may terminate this agreement for any reason on [TERMINATION NOTICE BUSINESS DAYS] Business Days’ notice to the other party."@en ;
                        rdfs:label "hasTerminationOnNotice"@en .


:hasWaiver rdfs:comment "The failure or neglect by a party to enforce any of rights under this agreement will not be deemed to be a waiver of that party's rights. "@en ;
           rdfs:label "hasWaiver"@en .


:license rdfs:label "License"@en .


:not_given rdfs:label "NotGiven"@en .


rdf:first rdfs:comment "The first item in the subject RDF list." ;
          rdfs:isDefinedBy rdf: ;
          rdfs:label "first" .


rdf:nil rdfs:comment "The empty list, with no items in it. If the rest of a list is nil then the list has no more items in it." ;
        rdfs:isDefinedBy rdf: ;
        rdfs:label "nil" .


rdf:object rdfs:comment "The object of the subject RDF statement." ;
           rdfs:isDefinedBy rdf: ;
           rdfs:label "object" .


rdf:predicate rdfs:comment "The predicate of the subject RDF statement." ;
              rdfs:isDefinedBy rdf: ;
              rdfs:label "predicate" .


rdf:rest rdfs:comment "The rest of the subject RDF list after the first item." ;
         rdfs:isDefinedBy rdf: ;
         rdfs:label "rest" .


rdf:subject rdfs:comment "The subject of the subject RDF statement." ;
            rdfs:isDefinedBy rdf: ;
            rdfs:label "subject" .


rdf:type rdfs:comment "The subject is an instance of a class." ;
         rdfs:isDefinedBy rdf: ;
         rdfs:label "type" .


rdf:value rdfs:comment "Idiomatic property used for structured values." ;
          rdfs:isDefinedBy rdf: ;
          rdfs:label "value" .


rdfs:domain rdfs:comment "A domain of the subject property." ;
            rdfs:isDefinedBy rdfs: ;
            rdfs:label "domain" .


rdfs:isDefinedBy rdfs:comment "The defininition of the subject resource." ;
                 rdfs:isDefinedBy rdfs: ;
                 rdfs:label "isDefinedBy" .


rdfs:label rdfs:comment "A human-readable name for the subject." ;
           rdfs:isDefinedBy rdfs: ;
           rdfs:label "label" .


rdfs:member rdfs:comment "A member of the subject resource." ;
            rdfs:isDefinedBy rdfs: ;
            rdfs:label "member" .


rdfs:range rdfs:comment "A range of the subject property." ;
           rdfs:isDefinedBy rdfs: ;
           rdfs:label "range" .


rdfs:seeAlso rdfs:comment "Further information about the subject resource." ;
             rdfs:isDefinedBy rdfs: ;
             rdfs:label "seeAlso" .


rdfs:subClassOf rdfs:comment "The subject is a subclass of a class." ;
                rdfs:isDefinedBy rdfs: ;
                rdfs:label "subClassOf" .


rdfs:subPropertyOf rdfs:comment "The subject is a subproperty of a property." ;
                   rdfs:isDefinedBy rdfs: ;
                   rdfs:label "subPropertyOf" .


owl:allValuesFrom rdfs:comment "The property that determines the class that a universal property restriction refers to." ;
                  rdfs:isDefinedBy owl: ;
                  rdfs:label "allValuesFrom" .


owl:annotatedProperty rdfs:comment "The property that determines the predicate of an annotated axiom or annotated annotation." ;
                      rdfs:isDefinedBy owl: ;
                      rdfs:label "annotatedProperty" .


owl:annotatedSource rdfs:comment "The property that determines the subject of an annotated axiom or annotated annotation." ;
                    rdfs:isDefinedBy owl: ;
                    rdfs:label "annotatedSource" .


owl:annotatedTarget rdfs:comment "The property that determines the object of an annotated axiom or annotated annotation." ;
                    rdfs:isDefinedBy owl: ;
                    rdfs:label "annotatedTarget" .


owl:assertionProperty rdfs:comment "The property that determines the predicate of a negative property assertion." ;
                      rdfs:isDefinedBy owl: ;
                      rdfs:label "assertionProperty" .


owl:complementOf rdfs:comment "The property that determines that a given class is the complement of another class." ;
                 rdfs:isDefinedBy owl: ;
                 rdfs:label "complementOf" .


owl:datatypeComplementOf rdfs:comment "The property that determines that a given data range is the complement of another data range with respect to the data domain." ;
                         rdfs:isDefinedBy owl: ;
                         rdfs:label "datatypeComplementOf" .


owl:disjointUnionOf rdfs:comment "The property that determines that a given class is equivalent to the disjoint union of a collection of other classes." ;
                    rdfs:isDefinedBy owl: ;
                    rdfs:label "disjointUnionOf" .


owl:disjointWith rdfs:comment "The property that determines that two given classes are disjoint." ;
                 rdfs:isDefinedBy owl: ;
                 rdfs:label "disjointWith" .


owl:distinctMembers rdfs:comment "The property that determines the collection of pairwise different individuals in a owl:AllDifferent axiom." ;
                    rdfs:isDefinedBy owl: ;
                    rdfs:label "distinctMembers" .


owl:equivalentClass rdfs:comment "The property that determines that two given classes are equivalent, and that is used to specify datatype definitions." ;
                    rdfs:isDefinedBy owl: ;
                    rdfs:label "equivalentClass" .


owl:equivalentProperty rdfs:comment "The property that determines that two given properties are equivalent." ;
                       rdfs:isDefinedBy owl: ;
                       rdfs:label "equivalentProperty" .


owl:hasKey rdfs:comment "The property that determines the collection of properties that jointly build a key." ;
           rdfs:isDefinedBy owl: ;
           rdfs:label "hasKey" .


owl:hasSelf rdfs:comment "The property that determines the property that a self restriction refers to." ;
            rdfs:isDefinedBy owl: ;
            rdfs:label "hasSelf" .


owl:hasValue rdfs:comment "The property that determines the individual that a has-value restriction refers to." ;
             rdfs:isDefinedBy owl: ;
             rdfs:label "hasValue" .


owl:intersectionOf rdfs:comment "The property that determines the collection of classes or data ranges that build an intersection." ;
                   rdfs:isDefinedBy owl: ;
                   rdfs:label "intersectionOf" .


owl:inverseOf rdfs:comment "The property that determines that two given properties are inverse." ;
              rdfs:isDefinedBy owl: ;
              rdfs:label "inverseOf" .


owl:members rdfs:comment "The property that determines the collection of members in either a owl:AllDifferent, owl:AllDisjointClasses or owl:AllDisjointProperties axiom." ;
            rdfs:isDefinedBy owl: ;
            rdfs:label "members" .


owl:onClass rdfs:comment "The property that determines the class that a qualified object cardinality restriction refers to." ;
            rdfs:isDefinedBy owl: ;
            rdfs:label "onClass" .


owl:onDataRange rdfs:comment "The property that determines the data range that a qualified data cardinality restriction refers to." ;
                rdfs:isDefinedBy owl: ;
                rdfs:label "onDataRange" .


owl:onDatatype rdfs:comment "The property that determines the datatype that a datatype restriction refers to." ;
               rdfs:isDefinedBy owl: ;
               rdfs:label "onDatatype" .


owl:onProperties rdfs:comment "The property that determines the n-tuple of properties that a property restriction on an n-ary data range refers to." ;
                 rdfs:isDefinedBy owl: ;
                 rdfs:label "onProperties" .


owl:onProperty rdfs:comment "The property that determines the property that a property restriction refers to." ;
               rdfs:isDefinedBy owl: ;
               rdfs:label "onProperty" .


owl:oneOf rdfs:comment "The property that determines the collection of individuals or data values that build an enumeration." ;
          rdfs:isDefinedBy owl: ;
          rdfs:label "oneOf" .


owl:propertyChainAxiom rdfs:comment "The property that determines the n-tuple of properties that build a sub property chain of a given property." ;
                       rdfs:isDefinedBy owl: ;
                       rdfs:label "propertyChainAxiom" .


owl:propertyDisjointWith rdfs:comment "The property that determines that two given properties are disjoint." ;
                         rdfs:isDefinedBy owl: ;
                         rdfs:label "propertyDisjointWith" .


owl:someValuesFrom rdfs:comment "The property that determines the class that an existential property restriction refers to." ;
                   rdfs:isDefinedBy owl: ;
                   rdfs:label "someValuesFrom" .


owl:targetValue rdfs:comment "The property that determines the value of a negative data property assertion." ;
                rdfs:isDefinedBy owl: ;
                rdfs:label "targetValue" .


owl:unionOf rdfs:comment "The property that determines the collection of classes or data ranges that build a union." ;
            rdfs:isDefinedBy owl: ;
            rdfs:label "unionOf" .


owl:versionInfo rdfs:comment "The annotation property that provides version information for an ontology or another OWL construct." ;
                rdfs:isDefinedBy owl: ;
                rdfs:label "versionInfo" .


owl:withRestrictions rdfs:comment "The property that determines the collection of facet-value pairs that define a datatype restriction." ;
                     rdfs:isDefinedBy owl: ;
                     rdfs:label "withRestrictions" .


<http://www.w3.org/ns/dcat#endDate> rdfs:comment "The end of the period."@en .


<http://www.w3.org/ns/dcat#startDate> rdfs:comment "The start of the period."@en .


<http://www.w3.org/ns/dpv-gdpr#A7-3> rdfs:label "A7-3 Right to Withdraw Consent"@en .


<https://spec.edmcouncil.org/fibo/ontology/FND/Agreements/Contracts/hasEffectiveDate> rdfs:comment """definition
indicates the date a contract, relationship, or policy comes into force"""@en ;
                                                                                      rdfs:label "hasEffectiveDate"@en .


<https://spec.edmcouncil.org/fibo/ontology/FND/Agreements/Contracts/hasExecutionDate> rdfs:comment """definition
indicates the date a contract has been signed by all the necessary parties
explanatory note
This may or may not be the 'effective date' of the contract, which may be specified in the body of the document."""@en ;
                                                                                      rdfs:label "hasExecutionDate"@en .


###  Generated by the OWL API (version 5.1.14) https://github.com/owlcs/owlapi/
